ARM_Monadic_Ops.thy
@@ -19929,6 +19929,8 @@ where
 }"
 
 
+
+
 ML \<open>
 local 
 open L3 
