MMU_Ops.thy
@@ -1,13 +1,17 @@
 theory MMU_Ops
+
 imports ARM_Monadic
+
 begin
+
 
 class mmu =
   fixes mmu_translate :: "vaddr \<Rightarrow> 'a state_scheme \<Rightarrow> paddr \<times> 'a state_scheme" 
 
-class mem_op = mmu +
-  fixes mmu_read :: "vaddr \<Rightarrow> 'a state_scheme \<Rightarrow> bool list \<times> 'a state_scheme"
-  fixes mmu_read_size :: "vaddr \<times> nat  \<Rightarrow> 'a state_scheme \<Rightarrow> bool list \<times> 'a state_scheme"
-  fixes mmu_write_size :: "bool list \<times> vaddr \<times> nat \<Rightarrow> 'a state_scheme \<Rightarrow> unit \<times> 'a state_scheme"
+
+class mem_op =
+  fixes mmu_read :: "vaddr \<Rightarrow> 'a::mmu state_scheme \<Rightarrow> bool list \<times> 'a::mmu state_scheme"
+  fixes mmu_read_size :: "vaddr \<times> nat  \<Rightarrow> 'a::mmu state_scheme \<Rightarrow> bool list \<times> 'a::mmu state_scheme"
+  fixes mmu_write_size :: "bool list \<times> vaddr \<times> nat \<Rightarrow> 'a::mmu state_scheme \<Rightarrow> unit \<times> 'a::mmu state_scheme"
 
 end
