MachineARM.thy
@@ -22,7 +22,7 @@
 *)
 
 theory MachineARM
-imports Pointers "Word_Lib/Word_Lib"
+imports Pointers "/home/hiras/nfshome/verification/l4v/lib/Word_Lib/Word_Lib"
 begin
 
 text {* Address types *}
