logic/Con_Set.thy
@@ -12,25 +12,34 @@ where
   "con_set V s \<equiv>  \<forall>va\<in>V. (asid s, va) \<notin> incon_set s"
 
 
-(* vcg check for the flush and con_set memory writes, in Kernel Mode  *)
+(* vcgm check for the flush and con_set memory writes, in Kernel Mode  *)
 
 lemma flush_TLB_mem_write':
   "\<Turnstile> \<lbrace> \<lambda>s. aval lval s = Some vp \<and> aval rval s = Some v \<and> vp \<notin> SA  \<and> con_set SA s \<and> mode s = Kernel \<and> 
       ptable_lift_m (heap s) (root s) (mode s) (Addr vp) = Some pp \<rbrace>  Flush flushTLB ;; lval ::= rval \<lbrace>\<lambda>s. heap s pp = Some v \<rbrace>"
-   by vcg
+   by vcgm
 
 
 lemma flush_ASID_mem_write':
   "\<Turnstile> \<lbrace> \<lambda>s. aval lval s = Some vp \<and> aval rval s = Some v \<and> asid s = a \<and>  vp \<notin> SA \<and> con_set SA s \<and> mode s = Kernel \<and> 
       ptable_lift_m (heap s) (root s) (mode s) (Addr vp) = Some pp \<rbrace>  Flush (flushASID a) ;; lval ::= rval \<lbrace>\<lambda>s. heap s pp = Some v \<rbrace>"
-  by vcg
+  by vcgm
+
+
+lemma [simp]:
+  " mem_read_hp' (asid sa) (incon_set sa) (heap sa) (root sa) (Addr x2) = Some v
+                \<Longrightarrow> mem_read_hp' (asid sa) {av \<in> incon_set sa. fst av \<noteq> s \<and> snd av \<noteq> vp} (heap sa) (root sa) (Addr x2) = Some v"
+ by (clarsimp simp: mem_read_hp'_def split: split_if_asm)
+
+lemma  [simp]:
+  "aval e sa = Some v \<Longrightarrow> aval e (sa\<lparr>incon_set := {av \<in> incon_set sa. fst av \<noteq> s \<and> snd av \<noteq> vp}\<rparr>) = Some v "
+  by (induct e arbitrary: v; clarsimp split: option.splits; fastforce)
 
 
 lemma flush_ASID_va_mem_write':
   "\<Turnstile> \<lbrace> \<lambda>s. aval lval s = Some vp \<and> aval rval s = Some v \<and> asid s = a \<and> vp \<notin> SA \<and> con_set SA s \<and> mode s = Kernel \<and> 
       ptable_lift_m (heap s) (root s) (mode s)(Addr vp) = Some pp \<rbrace>  Flush (flushASIDva s  (Addr vp)) ;; lval ::= rval \<lbrace>\<lambda>s. heap s pp = Some v \<rbrace>"
-   by vcg
-
+   by vcgm
 
 
 lemma [simp]:
