logic/MMU_Prg_Logic.thy
@@ -1,8 +1,9 @@
 theory MMU_Prg_Logic
 
-imports 
+imports
  "~~/src/HOL/Word/Word" "./../PageTable_seL4_m" "./../L3_Lib"
-        
+   "./../Rule_By_Method"
+
 
 begin
 
@@ -10,13 +11,13 @@ type_synonym val         = "32 word"
 type_synonym asid        = "8 word"
 type_synonym word_type   = "32 word"
 type_synonym heap        = "paddr \<rightharpoonup> 32 word"
-type_synonym rootreg     = "32 word"    (* should we take 32 word only as now we are abstracting logic 
+type_synonym rootreg     = "32 word"    (* should we take 32 word only as now we are abstracting logic
                                    without the details of machine *)
 type_synonym rt_map_t    = "paddr \<rightharpoonup> asid"
 
 datatype mode_t = Kernel | User
 
-datatype typ_tag'  = fst_lvl_pg_tbl | 
+datatype typ_tag'  = fst_lvl_pg_tbl |
                      snd_lvl_pg_tbl |
                      untype_mem
 
@@ -30,13 +31,13 @@ record p_state =
   tagged_heap :: heap_typ
   root_log :: "paddr set"
   root_map :: "paddr \<rightharpoonup> asid"       (* what about address sharing *)
-  asid  :: asid 
-  root :: "paddr" 
-  incon_set :: "(asid \<times> 32 word) set" 
-  mode :: mode_t  
-  
+  asid  :: asid
+  root :: "paddr"
+  incon_set :: "(asid \<times> 32 word) set"
+  mode :: mode_t
 
-definition 
+
+definition
   load_list_word_hp :: "heap \<Rightarrow> nat \<Rightarrow> paddr \<rightharpoonup> val list"
 where
   "load_list_word_hp h n p = load_list h n p"
@@ -46,27 +47,27 @@ definition
   from_word :: "32 word list => 'b :: len0 word" where
   "from_word \<equiv> word_rcat \<circ> rev"
 
-definition 
+definition
   load_value_word_hp :: "heap \<Rightarrow> paddr \<rightharpoonup> val"
 where
   "load_value_word_hp h p = map_option from_word (load_list_word_hp h 1 p)"
 
 
-definition 
+definition
   mem_read_word_heap :: "paddr \<Rightarrow> p_state \<rightharpoonup> word_type"
 where
   "mem_read_word_heap p s = load_value_word_hp (heap s) p "
-          
+
 
 definition
   decode_heap_pde' :: "heap \<Rightarrow> paddr \<rightharpoonup> pde" where
-  "decode_heap_pde' h p \<equiv> 
+  "decode_heap_pde' h p \<equiv>
      map_option decode_pde (h p)"
 
 definition
   get_pde' :: "heap \<Rightarrow> paddr \<Rightarrow> vaddr \<rightharpoonup> pde" where
   "get_pde' h rt vp \<equiv>
-     let 
+     let
        pd_idx_offset = ((vaddr_pd_index (addr_val vp)) << 2)
      in
        decode_heap_pde' h (rt r+ pd_idx_offset)"
@@ -78,9 +79,9 @@ definition
 
 definition
   get_pte' :: "heap \<Rightarrow> paddr \<Rightarrow> vaddr \<rightharpoonup> pte" where
-  "get_pte' h pt_base vp \<equiv> 
-     let 
-       pt_idx_offset = ((vaddr_pt_index (addr_val vp)) << 2) 
+  "get_pte' h pt_base vp \<equiv>
+     let
+       pt_idx_offset = ((vaddr_pt_index (addr_val vp)) << 2)
      in
        decode_heap_pte' h (pt_base r+ pt_idx_offset)"
 
@@ -90,7 +91,7 @@ definition
   where
   "lookup_pte' h pt_base vp \<equiv>
    case_option None
-    (\<lambda>pte. case pte 
+    (\<lambda>pte. case pte
              of InvalidPTE \<Rightarrow> None
               | SmallPagePTE base perms \<Rightarrow> Some (base, ArmSmallPage, perms))
     (get_pte' h pt_base vp)"
@@ -101,7 +102,7 @@ definition
   where
   "lookup_pde' h rt vp \<equiv>
    case_option None
-    (\<lambda>pde. case pde 
+    (\<lambda>pde. case pde
             of InvalidPDE \<Rightarrow> None
              | ReservedPDE \<Rightarrow> None
              | SectionPDE base perms \<Rightarrow> Some (base, ArmSection, perms)
@@ -115,8 +116,8 @@ definition
      let
        vp_val = addr_val vp
      in
-       map_option 
-         (\<lambda>(base, pg_size, perms). 
+       map_option
+         (\<lambda>(base, pg_size, perms).
              base r+ (vaddr_offset pg_size vp_val))
          (lookup_pde' h pt_root vp)"
 
@@ -124,13 +125,13 @@ definition
 definition
   mem_read_hp :: "heap \<Rightarrow> paddr \<Rightarrow> vaddr \<rightharpoonup> val"
 where
-  "mem_read_hp hp rt vp =  (ptable_lift' hp rt \<rhd>o load_value_word_hp hp) vp" 
+  "mem_read_hp hp rt vp =  (ptable_lift' hp rt \<rhd>o load_value_word_hp hp) vp"
 
 
 definition
   ptable_trace' :: "heap \<Rightarrow> paddr \<Rightarrow> vaddr \<Rightarrow> paddr set" where
   "ptable_trace' h rt vp \<equiv>
-     let 
+     let
        vp_val = addr_val vp ;
        pd_idx_offset = ((vaddr_pd_index vp_val) << 2) ;
        pt_idx_offset = ((vaddr_pt_index vp_val) << 2) ;
@@ -138,8 +139,8 @@ definition
        pt_touched = (\<lambda>pt_base. {pt_base r+ pt_idx_offset})
      in
       (case decode_heap_pde' h (rt r+ pd_idx_offset)
-         of Some pde \<Rightarrow> 
-              (case pde 
+         of Some pde \<Rightarrow>
+              (case pde
                  of PageTablePDE pt_base \<Rightarrow> pd_touched \<union> pt_touched pt_base
                   | _ \<Rightarrow> pd_touched)
           | None \<Rightarrow> {})"
@@ -147,7 +148,7 @@ definition
 definition
   pde_trace' :: "heap \<Rightarrow> paddr \<Rightarrow> vaddr \<rightharpoonup> paddr" where
   "pde_trace' h rt vp \<equiv>
-     let 
+     let
        vp_val = addr_val vp ;
        pd_idx_offset = ((vaddr_pd_index vp_val) << 2) ;
        pd_touched = rt r+ pd_idx_offset
@@ -172,8 +173,8 @@ lemma ptable_lift_preserved':
   apply (rule conjI)
    apply (rule_tac x = "(SmallPagePTE a b)" in exI, clarsimp simp: get_pte'_def decode_heap_pte'_def , clarsimp)
   by (case_tac x2 ; clarsimp simp:get_pte'_def decode_heap_pte'_def)
-  
-  
+
+
 
 
 lemma ptable_trace_preserved':
@@ -194,12 +195,12 @@ where
   "ptable_mapped h r  \<equiv>   {va. \<exists>p. ptable_lift' h r va = Some p \<and>  p \<in> \<Union>(ptable_trace' h r ` UNIV) } "
 
 
-definition 
-  "user_perms perms  = (arm_p_AP perms = 0x2 \<or> arm_p_AP perms = 0x3)" 
+definition
+  "user_perms perms  = (arm_p_AP perms = 0x2 \<or> arm_p_AP perms = 0x3)"
 
-definition 
-  "filter_pde  m =    (\<lambda>x. case x of None \<Rightarrow> None 
-                       |  Some (base, pg_size, perms) \<Rightarrow> 
+definition
+  "filter_pde  m =    (\<lambda>x. case x of None \<Rightarrow> None
+                       |  Some (base, pg_size, perms) \<Rightarrow>
                            if (m = Kernel) \<or> (m = User \<and> user_perms perms)
                             then Some (base, pg_size, perms)
                             else None) "
@@ -210,10 +211,10 @@ where
   "lookup_pde_perm h r m vp = filter_pde  m (lookup_pde' h r vp)"
 
 definition
-  ptable_lift_m :: "heap \<Rightarrow> paddr \<Rightarrow> mode_t \<Rightarrow> vaddr \<rightharpoonup> paddr" 
+  ptable_lift_m :: "heap \<Rightarrow> paddr \<Rightarrow> mode_t \<Rightarrow> vaddr \<rightharpoonup> paddr"
 where
   "ptable_lift_m h r m vp \<equiv>
-        map_option  (\<lambda>(base, pg_size, perms).  base r+ (vaddr_offset pg_size (addr_val vp))) 
+        map_option  (\<lambda>(base, pg_size, perms).  base r+ (vaddr_offset pg_size (addr_val vp)))
                       (lookup_pde_perm h r m vp) "
 
 
@@ -228,7 +229,7 @@ lemma  [simp]:
 
 
 lemma  ptable_lift_m_user [simp]:
-  " ptable_lift_m h r  User va = Some pa \<Longrightarrow> 
+  " ptable_lift_m h r  User va = Some pa \<Longrightarrow>
          ptable_lift_m h r  User va =  ptable_lift' h r va"
   by (clarsimp simp: ptable_lift_m_def ptable_lift'_def lookup_pde_perm_def filter_pde_def split: option.splits split_if_asm)
 
@@ -237,14 +238,14 @@ lemma  ptable_lift_m_user [simp]:
 lemma ptlift_trace_some':
   "ptable_lift_m h r m vp = Some pa \<Longrightarrow>  ptable_trace' h r vp \<noteq> {}"
   by (case_tac m , simp add:  ptlift_trace_some , simp, frule ptable_lift_m_user, simp add: ptlift_trace_some)
-  
+
 
 lemma ptable_trace_preserved_m:
   "\<lbrakk>ptable_lift_m h r m vp = Some pb; p \<notin> ptable_trace' h r vp;
         pa \<notin> ptable_trace' h r vp \<rbrakk>  \<Longrightarrow>  pa \<notin> ptable_trace' (h(p \<mapsto> v)) r vp"
   by (case_tac m ,simp add: ptable_trace_preserved', simp, frule ptable_lift_m_user, simp add: ptable_trace_preserved')
-  
-                     
+
+
 
 lemma ptable_lift_preserved_m:
   " \<lbrakk>p \<notin> ptable_trace' h r vp; ptable_lift_m h r m vp = Some pa\<rbrakk> \<Longrightarrow> ptable_lift_m (h(p \<mapsto> v)) r m vp = Some pa"
@@ -263,7 +264,7 @@ lemma ptable_lift_preserved_m:
 
 lemma ptable_lift_m_implies_ptlift:
   "ptable_lift_m (heap s) (root s) (mode s) (Addr vp) = Some p \<Longrightarrow> ptable_lift' (heap s) (root s) (Addr vp) = Some p"
-  by (clarsimp simp: ptable_lift_m_def ptable_lift'_def lookup_pde_perm_def filter_pde_def user_perms_def split: option.splits split_if_asm)   
+  by (clarsimp simp: ptable_lift_m_def ptable_lift'_def lookup_pde_perm_def filter_pde_def user_perms_def split: option.splits split_if_asm)
 
 
 lemma union_imp_all:
@@ -274,17 +275,17 @@ lemma union_imp_all:
 
 (* the following two definitions are not being used for the time being *)
 
-definition 
+definition
   update_mem_tag :: "heap_typ \<Rightarrow> paddr \<Rightarrow>  typ_tag \<Rightarrow> heap_typ"
 where
-  "update_mem_tag ht p t \<equiv>  ht (p := t) " 
+  "update_mem_tag ht p t \<equiv>  ht (p := t) "
 
 consts update_mem_tag_set :: "heap_typ \<Rightarrow> paddr set \<Rightarrow>  typ_tag \<Rightarrow> heap_typ"
 
-definition 
+definition
   update_mem_tag_set' :: "heap_typ \<Rightarrow> paddr set \<Rightarrow>  typ_tag \<Rightarrow> bool"
 where
-  "update_mem_tag_set' ht P t \<equiv> \<forall>x\<in>P. ht x = t" 
+  "update_mem_tag_set' ht P t \<equiv> \<forall>x\<in>P. ht x = t"
 
 
 
@@ -295,14 +296,14 @@ where
 definition
   first_level_defined_page_table :: "heap \<Rightarrow> heap_typ \<Rightarrow> paddr \<Rightarrow> bool"
 where
-  "first_level_defined_page_table  h ht r \<equiv> \<forall>v. \<exists>pde. get_pde' h r v = Some pde \<and> 
+  "first_level_defined_page_table  h ht r \<equiv> \<forall>v. \<exists>pde. get_pde' h r v = Some pde \<and>
                 (\<forall>x\<in>\<Union>(ptable_trace' h r ` UNIV). ht x = page_table)"
 
 
 definition
   page_tables_of_roots :: "heap \<Rightarrow> heap_typ \<Rightarrow> paddr set \<Rightarrow>  bool"
 where
-  "page_tables_of_roots h ht rset \<equiv> \<forall>r\<in>rset. \<forall>v. \<exists>pde. get_pde' h r v = Some pde \<and> 
+  "page_tables_of_roots h ht rset \<equiv> \<forall>r\<in>rset. \<forall>v. \<exists>pde. get_pde' h r v = Some pde \<and>
         (\<forall>x\<in>\<Union>(ptable_trace' h r ` UNIV). ht x = page_table)"
 
 
@@ -326,25 +327,25 @@ where
 
 (* may be remove later , if its giving problem in simp*)
 
-lemma [simp]: "current_page_table s =  (\<forall>v. \<exists>pde. get_pde' (heap s) (root s) v = Some pde \<and> 
+lemma [simp]: "current_page_table s =  (\<forall>v. \<exists>pde. get_pde' (heap s) (root s) v = Some pde \<and>
         (\<forall>x\<in>\<Union>(ptable_trace' (heap s) (root s) ` UNIV). (tagged_heap s) x = page_table))"
   by (clarsimp simp: current_page_table_def first_level_defined_page_table_def)
 
-lemma [simp]: "page_tables s = (\<forall>rt\<in>root_log s. \<forall>v. \<exists>pde. get_pde' (heap s) rt v = Some pde \<and> 
+lemma [simp]: "page_tables s = (\<forall>rt\<in>root_log s. \<forall>v. \<exists>pde. get_pde' (heap s) rt v = Some pde \<and>
                               (\<forall>x\<in>\<Union>(ptable_trace' (heap s) rt ` UNIV). (tagged_heap s) x = page_table))"
   by(clarsimp simp: page_tables_def page_tables_of_roots_def)
 
 
 
 
-(* assumption of non-sharing address space of the processes, pages can be shared, but even then every process will have its own 
+(* assumption of non-sharing address space of the processes, pages can be shared, but even then every process will have its own
           page table entry *)
 
 
 definition
   non_overlapping_page_tables_assertion :: "paddr set \<Rightarrow> heap \<Rightarrow> bool"
 where
-  "non_overlapping_page_tables_assertion rset h \<equiv>  
+  "non_overlapping_page_tables_assertion rset h \<equiv>
            (\<forall>x y. x\<in>rset \<and> y\<in>rset \<and> x\<noteq>y \<longrightarrow> \<Union>(ptable_trace' h x ` UNIV) \<inter> \<Union>(ptable_trace' h y ` UNIV) = {})"
 
 
@@ -358,22 +359,22 @@ where
 (* brackets might be an issue *)
 
 lemma [simp]:
-  "non_overlapping_page_tables s = ((\<forall>rt\<in>root_log s. (\<forall>v. \<exists>pde. get_pde' (heap s) rt v = Some pde) \<and> 
+  "non_overlapping_page_tables s = ((\<forall>rt\<in>root_log s. (\<forall>v. \<exists>pde. get_pde' (heap s) rt v = Some pde) \<and>
          (\<forall>a. \<forall>x\<in>ptable_trace' (heap s) rt a. tagged_heap s x = page_table)) \<and> non_overlapping_page_tables_assertion (root_log s) (heap s))"
   by (clarsimp simp: non_overlapping_page_tables_def)
 
-                      
+
 (* previous version, have to remove later *)
 
 definition
   non_overlapping_page_tables' :: "p_state \<Rightarrow> bool"
 where
-  "non_overlapping_page_tables' s \<equiv> (\<forall>rt\<in>root_log s. \<forall>v. \<exists>pde. get_pde' (heap s) rt v = Some pde \<and> 
-                                  (\<forall>x\<in>\<Union>(ptable_trace' (heap s) rt ` UNIV). (tagged_heap s) x = page_table)) \<and> 
+  "non_overlapping_page_tables' s \<equiv> (\<forall>rt\<in>root_log s. \<forall>v. \<exists>pde. get_pde' (heap s) rt v = Some pde \<and>
+                                  (\<forall>x\<in>\<Union>(ptable_trace' (heap s) rt ` UNIV). (tagged_heap s) x = page_table)) \<and>
              (\<forall>x y. x\<in>root_log s \<and> y\<in>root_log s \<and> x\<noteq>y \<longrightarrow> \<Union>(ptable_trace' (heap s) x ` UNIV) \<inter> \<Union>(ptable_trace' (heap s) y ` UNIV) = {})"
 
 
-(* range of virtual addresses mapped by a section entry , entry can be valid or invalid  
+(* range of virtual addresses mapped by a section entry , entry can be valid or invalid
   we might use this in the flush by vaddr set
    is there any better way of stating this, like ran or dom ? *)
 
