logic/Mode_Switch.thy
@@ -1,20 +1,20 @@
 theory Mode_Switch
-                  
+
 imports Memory_Model
-        
-
-begin               
 
 
-declare assign_sound [vcg del] 
+begin
 
-(* 
-there is a need of a memory model now, a typed memory, that 
-explicitly differentiate between page tables and rest of the memory  
+
+declare assign_sound [vcg del]
+
+(*
+there is a need of a memory model now, a typed memory, that
+explicitly differentiate between page tables and rest of the memory
 *)
 
-(*   
-first theorem, kernel wrote to the memory but it didn't change the page tables at all, then there should not be TLB flush, 
+(*
+first theorem, kernel wrote to the memory but it didn't change the page tables at all, then there should not be TLB flush,
 here we should only tag the heap with page_tables, lets gp ans see the program state
 
 *)
@@ -22,10 +22,10 @@ here we should only tag the heap with page_tables, lets gp ans see the program s
 definition
   kernel_state :: "p_state \<Rightarrow> bool"
 where
-  "kernel_state s \<equiv>     \<exists>rt a. root s = rt  \<and> mode s = Kernel \<and> 
+  "kernel_state s \<equiv>     \<exists>rt a. root s = rt  \<and> mode s = Kernel \<and>
                         asid s = a  \<and> root_map s rt = Some a \<and> partial_inj (root_map s) \<and> rt\<in>root_log s \<and>
                         global_mappings_of_all_processes s \<and> non_overlapping_page_tables s  \<and>
-                        \<Union>(ptable_trace' (heap s) (root s) ` UNIV) \<subseteq> kernel_phy_mem" 
+                        \<Union>(ptable_trace' (heap s) (root s) ` UNIV) \<subseteq> kernel_phy_mem"
 
 
 lemma kernel_state_implies_current_page_table:
@@ -43,7 +43,7 @@ done
 (* when kernel doesn't write to any of the page-table *)
 
 lemma [simp]:
-  "\<lbrakk>kernel_state s; assigned_asids_consistent (root_map s) (incon_set s)\<rbrakk> \<Longrightarrow> 
+  "\<lbrakk>kernel_state s; assigned_asids_consistent (root_map s) (incon_set s)\<rbrakk> \<Longrightarrow>
                     con_set VA s"
   apply (clarsimp simp: assigned_asids_consistent_def con_set_def kernel_state_def assigned_asid_va_map_def ran_def)
   by force
@@ -55,9 +55,9 @@ lemma [simp]:
 
 
 lemma global_mappings_decode':
-  "\<lbrakk>kernel_state s  ; va \<in> kernel_safe_region' s\<rbrakk> \<Longrightarrow> 
+  "\<lbrakk>kernel_state s  ; va \<in> kernel_safe_region' s\<rbrakk> \<Longrightarrow>
          \<exists>p perm. decode_heap_pde' (heap s) (root s r+ (vaddr_pd_index va << 2)) =  Some (SectionPDE p perm)"
-  apply (clarsimp simp: kernel_safe_region'_def vas_mapped_by_global_mappings_def global_mappings_of_all_processes_def global_mappings_def 
+  apply (clarsimp simp: kernel_safe_region'_def vas_mapped_by_global_mappings_def global_mappings_of_all_processes_def global_mappings_def
                         pd_idx_offset_def get_pde'_def kernel_state_def)
   by force
 
@@ -79,11 +79,11 @@ lemma kernel_state_mode:
 
 lemma  mode_switch_safe_set_when_not_in_current_page_table:
   "\<Turnstile> \<lbrace> \<lambda>s. kernel_state s \<and> aval lval s = Some vp \<and> aval rval s = Some v \<and> vp \<in> SM \<and> SM = kernel_safe_region' s \<and>
-           assigned_asids_consistent (root_map s) (incon_set s)  \<and> 
+           assigned_asids_consistent (root_map s) (incon_set s)  \<and>
             (Addr vp r- global_offset) \<notin> \<Union>(ptable_trace' (heap s) (root s) ` UNIV) \<rbrace>
                      lval ::= rval ;; SetMode User
                   \<lbrace>\<lambda>s. safe_set (SM_user (heap s) (root s)) s \<and>  heap s (Addr vp r- global_offset) = Some v\<rbrace>"
-  apply_trace (vcg vcg: weak_pre_write [of SM])
+  apply (vcgm vcg: weak_pre_write [of SM])
   apply (rule conjI)
    apply (clarsimp simp: safe_set_def safe_memory_def ptrace_set_def)
   apply (rule conjI)
@@ -97,11 +97,11 @@ lemma  mode_switch_safe_set_when_not_in_current_page_table:
 
 lemma  mode_switch_invariant_for_current_asid:
   "\<Turnstile> \<lbrace> \<lambda>s. kernel_state s \<and> aval lval s = Some vp \<and> aval rval s = Some v \<and> vp \<in> SM \<and> SM = kernel_safe_region' s \<and>
-           assigned_asids_consistent (root_map s) (incon_set s)  \<and> 
+           assigned_asids_consistent (root_map s) (incon_set s)  \<and>
             (Addr vp r- global_offset) \<notin> \<Union>(ptable_trace' (heap s) (root s) ` UNIV) \<rbrace>
                      lval ::= rval ;; SetMode User
                   \<lbrace>\<lambda>s. {asid s} \<times> UNIV  \<inter> incon_set s = {}\<rbrace>"
-  apply_trace (vcg vcg: assign_sound)
+  apply (vcgm vcg: assign_sound)
   apply (rule conjI)
    apply (clarsimp simp: assigned_asids_consistent_def assigned_asid_va_map_def ran_def kernel_state_def)
    apply force
@@ -109,7 +109,7 @@ lemma  mode_switch_invariant_for_current_asid:
    apply (clarsimp simp: kernel_state_def)
   apply (clarsimp simp: pde_comp_empty)
   apply (clarsimp simp: assigned_asids_consistent_def assigned_asid_va_map_def ran_def kernel_state_def)
-  by auto                                 
+  by auto
 
 
 (* might not a be a good use case *)
@@ -118,10 +118,10 @@ lemma  mode_switch_invariant_for_current_asid:
 
 lemma mode_switch_safe_set_when_not_in_page_table:
   "\<Turnstile> \<lbrace> \<lambda>s. kernel_state s \<and> aval lval s = Some vp \<and> aval rval s = Some v \<and> vp \<in> SM \<and> SM = kernel_safe_region' s \<and>
-             assigned_asids_consistent (root_map s) (incon_set s)  \<and> (tagged_heap s) (Addr vp r- global_offset) \<noteq> page_table \<rbrace> 
+             assigned_asids_consistent (root_map s) (incon_set s)  \<and> (tagged_heap s) (Addr vp r- global_offset) \<noteq> page_table \<rbrace>
                      lval ::= rval ;; SetMode User
                   \<lbrace>\<lambda>s. safe_set (SM_user (heap s) (root s)) s \<and>  heap s (Addr vp r- global_offset) = Some v\<rbrace>"
-  apply_trace (vcg vcg: weak_pre_write [of SM])
+  apply (vcgm vcg: weak_pre_write [of SM])
   apply (frule kernel_state_implies_page_tables)
   apply (rule conjI)
    apply (clarsimp simp: safe_set_def safe_memory_def ptrace_set_def)
@@ -138,10 +138,10 @@ done
 
 lemma mode_switch_invariant_for_all_assigned_asid:
   "\<Turnstile> \<lbrace> \<lambda>s. kernel_state s \<and> aval lval s = Some vp \<and> aval rval s = Some v \<and> vp \<in> SM \<and> SM = kernel_safe_region' s \<and>
-             assigned_asids_consistent (root_map s) (incon_set s)  \<and> (tagged_heap s) (Addr vp r- global_offset) \<noteq> page_table \<rbrace> 
+             assigned_asids_consistent (root_map s) (incon_set s)  \<and> (tagged_heap s) (Addr vp r- global_offset) \<noteq> page_table \<rbrace>
                      lval ::= rval ;; SetMode User
                   \<lbrace>\<lambda>s. assigned_asids_consistent (root_map s) (incon_set s) \<rbrace>"
-  apply_trace (vcg vcg:  assign_sound)
+  apply (vcgm vcg:  assign_sound)
   apply (rule conjI)
    apply (clarsimp simp: assigned_asids_consistent_def assigned_asid_va_map_def ran_def kernel_state_def)
    apply force
@@ -160,11 +160,11 @@ done
 
 lemma mode_switch_safe_set_in_current_page_table:
   "\<Turnstile> \<lbrace> \<lambda>s. kernel_state s \<and> aval lval s = Some vp \<and> aval rval s = Some v \<and> vp \<in> SM \<and> SM = kernel_safe_region' s \<and>
-      assigned_asids_consistent (root_map s) (incon_set s)  \<and> 
+      assigned_asids_consistent (root_map s) (incon_set s)  \<and>
             Addr vp \<in> ptable_mapped (heap s) (root s) \<and> asid s = a \<rbrace>
                      lval ::= rval ;; Flush (flushASID a) ;; SetMode User
                   \<lbrace>\<lambda>s. safe_set (SM_user (heap s) (root s)) s  \<and> heap s (Addr vp r- global_offset) = Some v\<rbrace>"
-  apply_trace (vcg vcg: weak_pre_write [of SM])
+  apply (vcgm vcg: weak_pre_write [of SM])
   apply (rule conjI)
    apply (clarsimp simp: safe_set_def safe_memory_def ptrace_set_def)
   apply (rule conjI)
@@ -177,11 +177,11 @@ lemma mode_switch_safe_set_in_current_page_table:
 
 lemma  mode_switch_invariant_flush_current_asid:
   "\<Turnstile> \<lbrace> \<lambda>s. kernel_state s \<and> aval lval s = Some vp \<and> aval rval s = Some v \<and> vp \<in> SM \<and> SM = kernel_safe_region' s \<and>
-         assigned_asids_consistent (root_map s) (incon_set s)  \<and> 
+         assigned_asids_consistent (root_map s) (incon_set s)  \<and>
             Addr vp \<in> ptable_mapped (heap s) (root s) \<and> asid s = a \<rbrace>
                      lval ::= rval ;; Flush (flushASID a) ;; SetMode User
                   \<lbrace>\<lambda>s. {asid s} \<times> UNIV  \<inter> incon_set s = {}\<rbrace>"
-  apply_trace (vcg vcg:  assign_sound)
+  apply (vcgm vcg:  assign_sound)
   apply (rule conjI)
    apply (clarsimp simp: assigned_asids_consistent_def assigned_asid_va_map_def ran_def kernel_state_def)
    apply force
@@ -190,16 +190,11 @@ lemma  mode_switch_invariant_flush_current_asid:
   by force
 
 
-lemma
-  "fst av \<noteq> a  \<Longrightarrow> av \<notin> pde_comp a h1 h2 r"
-  apply (clarsimp simp: pde_comp_def)
-done
-
 
 lemma pde_comp_asid_incon:
-  "{av. (av \<in> incon_set s \<or> av \<in> pde_comp (asid s) (heap s) (heap s(Addr (vp - global_offset) \<mapsto> v)) (root s)) \<and> fst av \<noteq> asid s} =
+  "{av. (av \<in> incon_set s \<or> av \<in> pde_comp' (asid s) (heap s) (heap s(Addr (vp - global_offset) \<mapsto> v)) (root s)) \<and> fst av \<noteq> asid s} =
    {av. av \<in> incon_set s  \<and> fst av \<noteq> asid s}"
-  apply (clarsimp simp: pde_comp_def)
+  apply (clarsimp simp: pde_comp'_def)
   apply force
 done
 
@@ -211,7 +206,7 @@ lemma  mode_switch_invariant_flush_all_assigned_asid:
          assigned_asids_consistent (root_map s) (incon_set s)  \<and>  Addr vp \<in> ptable_mapped (heap s) (root s) \<and> asid s = a \<rbrace>
                      lval ::= rval ;; Flush (flushASID a) ;; SetMode User
                   \<lbrace>\<lambda>s. assigned_asids_consistent (root_map s) (incon_set s) \<rbrace>"
-  apply_trace (vcg vcg:  assign_sound)
+  apply (vcgm vcg:  assign_sound)
   apply (rule conjI)
    apply (clarsimp simp: assigned_asids_consistent_def assigned_asid_va_map_def ran_def kernel_state_def)
    apply force
@@ -242,7 +237,7 @@ lemma pde_comp_simp_vset_flush:
 done
 
 lemma incon_set_flsuhVA_section_simp:
-  "{asid s} \<times> UNIV \<inter> incon_set s = {} \<Longrightarrow> 
+  "{asid s} \<times> UNIV \<inter> incon_set s = {} \<Longrightarrow>
        {asid s} \<times> UNIV \<inter> {av \<in> incon_set s. snd av \<notin> addr_val ` vspace_section_entry (heap s) (root s) (SectionPDE p p_bits)} = {}"
   apply force
 done
@@ -254,20 +249,20 @@ lemma  remaining:
                (\<exists>p p_bits. get_pde' (heap s) (root s) (Addr vp) = Some (SectionPDE p p_bits) \<and> V = vspace_section_entry (heap s) (root s) (SectionPDE p p_bits) ) \<rbrace>
                                lval ::= rval ;; Flush (flushvarange V) ;; SetMode User
                   \<lbrace>\<lambda>s. {asid s} \<times> UNIV \<inter> incon_set s = {}\<rbrace>"
-  apply_trace (vcg vcg:  assign_sound)
+  apply (vcgm vcg:  assign_sound)
   apply (rule conjI)
    apply (clarsimp simp: assigned_asids_consistent_def assigned_asid_va_map_def ran_def  kernel_state_def)
    apply force
   apply (rule conjI)
    apply (clarsimp simp: kernel_state_def)
-  apply (subgoal_tac "pde_comp (asid s) (heap s) (heap s(Addr (vp - global_offset) \<mapsto> v)) (root s) =
+  apply (subgoal_tac "pde_comp' (asid s) (heap s) (heap s(Addr (vp - global_offset) \<mapsto> v)) (root s) =
                 (\<lambda>x. (asid s, addr_val x)) ` vspace_section_entry (heap s) (root s) (SectionPDE p p_bits) \<or>
-               pde_comp (asid s) (heap s) (heap s(Addr (vp - global_offset) \<mapsto> v)) (root s) = {}")
+               pde_comp' (asid s) (heap s) (heap s(Addr (vp - global_offset) \<mapsto> v)) (root s) = {}")
    apply (erule disjE)
     apply (clarsimp simp: pde_comp_simp_vset_flush)
     apply (rule incon_set_flsuhVA_section_simp , clarsimp simp: kernel_state_def
                 assigned_asids_consistent_def assigned_asid_va_map_def ran_def)
-    apply force
+(*    apply force
    apply (clarsimp simp: kernel_state_def assigned_asids_consistent_def assigned_asid_va_map_def ran_def)
    apply fastforce
   apply (case_tac "(heap s(Addr (vp - global_offset) \<mapsto> v)) (Addr (vp - global_offset)) = heap s (Addr (vp - global_offset))")
@@ -286,19 +281,19 @@ lemma  remaining:
    apply safe
   (*  here *)
   (* discuss with Gerwin, reasoning can be done but a little bit tricky, this theorem worth to spend time on?  *)
-
+  *)
 oops
 
 
 (* invariant preserved *)
 
-lemma 
+lemma
   "\<Turnstile> \<lbrace> \<lambda>s. kernel_state s \<and> aval lval s = Some vp \<and> aval rval s = Some v \<and> vp \<in> SM \<and> SM = kernel_safe_region' s \<and>
       assigned_asids_consistent (root_map s) (incon_set s)  \<and>  Addr vp \<in> ptable_mapped (heap s) (root s) \<and>
                (\<exists>p p_bits. get_pde' (heap s) (root s) (Addr vp) = Some (SectionPDE p p_bits) \<and> V = vspace_section_entry (heap s) (root s) (SectionPDE p p_bits) ) \<rbrace>
                                lval ::= rval ;; Flush (flushvarange V) ;; SetMode User
                   \<lbrace>\<lambda>s. safe_set (SM_user (heap s) (root s)) s \<and>  heap s (Addr vp r- global_offset) = Some v\<rbrace>"
-  apply_trace (vcg vcg: weak_pre_write [of SM])
+  apply (vcgm vcg: weak_pre_write [of SM])
   apply (rule conjI)
    apply (clarsimp simp: safe_set_def safe_memory_def ptrace_set_def)
   apply (rule conjI)
@@ -311,7 +306,7 @@ lemma
    apply (clarsimp simp: kernel_state_def assigned_asids_consistent_def assigned_asid_va_map_def ran_def)
    apply fastforce
  (* remaining, can be done but it requires reasoning *)
-   
+
 oops
 
 
@@ -343,18 +338,18 @@ lemma non_overlapping_page_tables_ptrace:
 
 lemma kernel_writing_to_inactive_process_page_table_and_flush:
   "\<Turnstile> \<lbrace> \<lambda>s. kernel_state s \<and> aval lval s = Some vp \<and> aval rval s = Some v \<and> vp \<in> SM \<and> SM = kernel_safe_region' s \<and>
-         assigned_asids_consistent (root_map s) (incon_set s)  \<and> rt \<in> root_log s \<and> rt \<noteq> root s \<and> 
+         assigned_asids_consistent (root_map s) (incon_set s)  \<and> rt \<in> root_log s \<and> rt \<noteq> root s \<and>
                   Addr vp r- global_offset \<in> \<Union>(ptable_trace' (heap s) rt ` UNIV) \<and> root_map s rt = Some a \<rbrace>
                      lval ::= rval ;; Flush (flushASID a) ;; SetMode User
                   \<lbrace>\<lambda>s. assigned_asids_consistent (root_map s) (incon_set s) \<rbrace>"
-  apply_trace (vcg vcg:  assign_sound)
+  apply (vcgm vcg:  assign_sound)
   apply (rule conjI)
    apply (clarsimp simp: assigned_asids_consistent_def  assigned_asid_va_map_def ran_def kernel_state_def)
    apply auto [1]
   apply (rule conjI)
    apply (clarsimp simp: kernel_state_def)
-  find_theorems "pde_comp"
-  apply (subgoal_tac "pde_comp (asid s) (heap s) (heap s(Addr (vp - global_offset) \<mapsto> v)) (root s) = {}")
+  find_theorems "pde_comp'"
+  apply (subgoal_tac "pde_comp' (asid s) (heap s) (heap s(Addr (vp - global_offset) \<mapsto> v)) (root s) = {}")
    apply clarsimp
    apply (clarsimp simp: assigned_asids_consistent_def)
    apply force
@@ -369,12 +364,12 @@ lemma kernel_writing_to_inactive_process_page_table_and_flush:
 (* update root register to an assigned root, that also has an assigned asid  *)
 
 
-lemma  context_swtich_to_assigned_root_valid_asid: 
+lemma  context_swtich_to_assigned_root_valid_asid:
   "\<Turnstile> \<lbrace> \<lambda>s. kernel_state s \<and> aval rt s = Some r \<and> Addr r \<in> root_log s \<and> root_map s (Addr r) = Some a \<and>
             assigned_asids_consistent (root_map s) (incon_set s) \<rbrace>
-                      UpdateTTBR0 rt ;; UpdateASID a 
+                      UpdateTTBR0 rt ;; UpdateASID a
                   \<lbrace>\<lambda>s. assigned_asids_consistent (root_map s) (incon_set s) \<rbrace>"
-  apply vcg
+  apply vcgm
   by (clarsimp simp: kernel_state_def)
 
 
@@ -385,7 +380,7 @@ definition
 
 lemma [simp]:
   "\<forall>rts. root_map s rts  \<noteq> Some a \<Longrightarrow>  a \<notin> ran (root_map s)"
-  by (simp add: ran_def) 
+  by (simp add: ran_def)
 
 
 lemma parital_inj_update:
@@ -398,9 +393,9 @@ lemma parital_inj_update:
 lemma context_switch:
   "\<Turnstile> \<lbrace> \<lambda>s. kernel_state s \<and> aval rt s = Some r \<and> Addr r \<in> root_log s \<and> root_map s (Addr r) = None \<and> (\<forall>rts. root_map s rts \<noteq> Some a) \<and>
             asid_assumption s \<rbrace>
-                       UpdateRTMap rt a ;; UpdateTTBR0 rt ;; UpdateASID a 
+                       UpdateRTMap rt a ;; UpdateTTBR0 rt ;; UpdateASID a
                   \<lbrace>\<lambda>s. assigned_asids_consistent (root_map s) (incon_set s) \<and> partial_inj (root_map s)\<rbrace>"
-  apply_trace (vcg vcg: rt_map_update_partial)
+  apply (vcgm vcg: rt_map_update_partial)
   (* how to use rt_map_update_partial with vcg *)
   apply (rule conjI)
    apply (clarsimp simp: kernel_state_def)
@@ -415,30 +410,30 @@ done
 
 (* map, remap and unmap  *)
 
-(*  transition in map    : invalid to valid (no flush/invalidate) 
+(*  transition in map    : invalid to valid (no flush/invalidate)
                   remap  : valid to valid   (flush by asid/VA range)
                   unmap  : valid yo invalid (flush by asid/VA range)
   *)
 
 
-thm pde_comp_def
+thm pde_comp'_def
 
-(*definition 
+(*definition
   pde_comp_n :: "asid \<Rightarrow> heap \<Rightarrow> heap \<Rightarrow> paddr \<Rightarrow> (asid \<times> 32 word) set"
 where
-  "pde_comp_n a hp1 hp2 rt \<equiv> 
-         (\<lambda>x. (a, addr_val x)) ` {va. (\<exists>p1 p2. ptable_lift' hp1 rt va = Some p1 \<and> ptable_lift' hp2 rt va = Some p2 \<and> p1 \<noteq> p2 )   
+  "pde_comp_n a hp1 hp2 rt \<equiv>
+         (\<lambda>x. (a, addr_val x)) ` {va. (\<exists>p1 p2. ptable_lift' hp1 rt va = Some p1 \<and> ptable_lift' hp2 rt va = Some p2 \<and> p1 \<noteq> p2 )
    (* it won't flush  if it re-maps the page to itself, this might not be consistent with seL4, there is some PR though *)
                                    \<or>  (\<exists>p. ptable_lift' hp1 rt va = Some p \<and> ptable_lift' hp2 rt va = None )}"
 *)
 (* pde_comp will work in the case of map and remap, but not in the case of unmap, because pde_comp will still be empty *)
 
-(*  Mapping *)                                                             
-        
+(*  Mapping *)
+
 thm get_pde'_def
 
 lemma ptrace_invalid_ptable_lift_none:
-  "\<lbrakk>p \<in> ptable_trace' h r v; h p = Some w; decode_pde w = InvalidPDE \<or> decode_pte_small w = InvalidPTE\<rbrakk>   \<Longrightarrow>  
+  "\<lbrakk>p \<in> ptable_trace' h r v; h p = Some w; decode_pde w = InvalidPDE \<or> decode_pte_small w = InvalidPTE\<rbrakk>   \<Longrightarrow>
         ptable_lift'  h r v = None"
   apply (clarsimp simp: ptable_trace'_def Let_def decode_heap_pde'_def split: option.splits)
   apply (case_tac "decode_pde x2" ; clarsimp)
@@ -467,28 +462,28 @@ done
 
 
 
-thm pde_comp_def
+thm pde_comp'_def
 (* true only for remap *)
-lemma        
-  "pde_comp a h (h(p \<mapsto> v)) r = {a} \<times> addr_val `{va. p \<in> ptable_trace' h t va}"
-  apply (clarsimp simp: pde_comp_def ptable_trace'_def Let_def)
+lemma
+  "pde_comp' a h (h(p \<mapsto> v)) r = {a} \<times> addr_val `{va. p \<in> ptable_trace' h t va}"
+  apply (clarsimp simp: pde_comp'_def ptable_trace'_def Let_def)
 oops
 
 lemma ptable_trace_get_pde:
-  "\<lbrakk>p \<notin> ptable_trace' h r x;  get_pde' h r x = Some pde\<rbrakk>  \<Longrightarrow> 
+  "\<lbrakk>p \<notin> ptable_trace' h r x;  get_pde' h r x = Some pde\<rbrakk>  \<Longrightarrow>
                    get_pde' (h(p \<mapsto> v)) r x = Some pde"
   apply (clarsimp simp: ptable_trace'_def Let_def get_pde'_def decode_heap_pde'_def )
   by (case_tac " decode_pde z" ; clarsimp)
 
 
 lemma ptable_trace_get_pte:
-  "\<lbrakk>p \<notin> ptable_trace' h r x;  get_pde' h r x = Some (PageTablePDE x3) ; get_pte' h x3 x = Some x2\<rbrakk> \<Longrightarrow> 
+  "\<lbrakk>p \<notin> ptable_trace' h r x;  get_pde' h r x = Some (PageTablePDE x3) ; get_pte' h x3 x = Some x2\<rbrakk> \<Longrightarrow>
              get_pte' (h(p \<mapsto> v)) x3 x = Some x2"
   apply (subgoal_tac "get_pde' (h(p \<mapsto> v)) r x = Some (PageTablePDE x3)")
    prefer 2
    apply (clarsimp simp: ptable_trace_get_pde)
   by (clarsimp simp: ptable_trace'_def Let_def get_pde'_def get_pte'_def decode_heap_pde'_def decode_heap_pte'_def)
-  
+
 
 lemma ptable_trace_lookup_pte:
   "\<lbrakk>p \<notin> ptable_trace' h r x;  get_pde' h r x = Some (PageTablePDE x3); lookup_pte' (h(p \<mapsto> v)) x3 x = None\<rbrakk> \<Longrightarrow>
@@ -496,75 +491,113 @@ lemma ptable_trace_lookup_pte:
   apply (clarsimp simp: lookup_pte'_def  Let_def)
   apply (clarsimp split: option.splits)
    by (clarsimp simp: ptable_trace_get_pte)+
- 
 
 
-lemma   map_pde_comp_empty:     
-  "h p = Some w \<and> (decode_pde w = InvalidPDE \<or> decode_pte_small w = InvalidPTE) \<Longrightarrow>  
-         pde_comp a h (h(p \<mapsto> v)) r = {}"
-  apply (clarsimp simp: pde_comp_def)
+lemma
+  " \<lbrakk>h p = Some w; decode_pde w = InvalidPDE\<rbrakk> \<Longrightarrow> is_fault (pt_walk a h r x)"
+  apply (clarsimp simp: pt_walk_def is_fault_def get_pde'_def decode_heap_pde'_def Let_def  vaddr_pd_index_def mask_def
+                  split:option.splits pde.splits pte.splits split_if_asm)
+  apply safe
+
+
+
+oops
+
+lemma rewrite_or:
+  "(\<not> P \<Longrightarrow> \<not>Q \<Longrightarrow> R) \<Longrightarrow> P \<or> Q \<or> R"
+   by auto
+
+
+
+lemma is_fault_pt_trace:
+   "\<not> is_fault (pt_walk a h r x) \<Longrightarrow> ptable_trace' h r x \<noteq> {}"
+   by (clarsimp simp: pt_walk_def is_fault_def ptable_trace'_def Let_def get_pde'_def split:option.splits pde.splits)
+
+find_theorems "ptable_trace'"
+
+
+lemma  pt_walk_preserved':
+  "\<lbrakk>p \<notin> ptable_trace' h r x; \<not> is_fault (pt_walk a h r x) \<rbrakk> \<Longrightarrow>
+       pt_walk a h r x = pt_walk a (h(p \<mapsto> v)) r x"
+  apply (frule is_fault_pt_trace)
+  apply (clarsimp simp: pt_walk_def is_fault_def  lookup_pde'_def get_pde'_def ptable_trace'_def Let_def split: option.splits)
+  apply (case_tac x2; clarsimp simp: decode_heap_pde'_def lookup_pte'_def split: option.splits)
+  apply (case_tac x2a ; clarsimp)
   apply (rule conjI)
-   apply clarsimp
+   apply (rule_tac x = "(SmallPagePTE x21 x22)" in exI, clarsimp simp: get_pte'_def decode_heap_pte'_def , clarsimp)
+  by (case_tac x2 ; clarsimp simp:get_pte'_def decode_heap_pte'_def)
+
+
+
+lemma ptrace_invalid_pt_walk_is_fault:
+  "\<lbrakk>p \<in> ptable_trace' h r v; h p = Some w; decode_pde w = InvalidPDE \<or> decode_pte_small w = InvalidPTE \<rbrakk>   \<Longrightarrow>
+        is_fault (pt_walk a h r v)"
+  apply (clarsimp simp: ptable_trace'_def Let_def decode_heap_pde'_def split: option.splits)
+  apply (case_tac "decode_pde x2" ; clarsimp)
+     apply (clarsimp simp: is_fault_def pt_walk_def  get_pde'_def decode_heap_pde'_def)
+    apply (clarsimp simp: is_fault_def pt_walk_def  get_pde'_def decode_heap_pde'_def)
+   prefer 2
+   apply (clarsimp simp: decode_pde_def decode_pte_small_def)
+  apply (erule_tac P = "p = x3 r+ (vaddr_pt_index (addr_val v) << 2)" in disjE)
+   apply (erule disjE)
+    prefer 2
+    apply (clarsimp simp: decode_pde_def decode_pte_small_def)
+   apply (clarsimp simp: is_fault_def pt_walk_def  get_pde'_def decode_heap_pde'_def lookup_pte'_def get_pte'_def decode_heap_pte'_def decode_pte_def)
+   apply (case_tac "decode_pte_small w")
+    apply clarsimp
+   apply (clarsimp simp: decode_pde_def Let_def decode_pte_small_def decode_pde_pt_def) apply (clarsimp split: split_if_asm)
+        apply (clarsimp simp:  decode_pde_pt_def)
+       apply (clarsimp simp: decode_pde_section_def)
+      apply word_bitwise apply force
+     apply (clarsimp simp: decode_pde_section_def)
+    apply (clarsimp simp: decode_pde_section_def)
+   apply word_bitwise apply force
+  by (clarsimp simp: decode_pde_def decode_pte_small_def Let_def)
+
+lemma
+  "\<lbrakk> \<not> is_fault (pt_walk a h r x); pt_walk a h r x = pt_walk a (h(p \<mapsto> v)) r x\<rbrakk>   \<Longrightarrow>
+       \<not> is_fault (pt_walk a (h(p \<mapsto> v)) r x)"
+
+
+oops
+
+lemma   map_pde_comp_empty:
+  "h p = Some w \<and> (decode_pde w = InvalidPDE \<or> decode_pte_small w = InvalidPTE) \<Longrightarrow>
+         pde_comp' a h (h(p \<mapsto> v)) r = {}"
+  apply (clarsimp simp: pde_comp'_def)
+  apply (rule conjI)
    apply (case_tac "p \<notin> ptable_trace' h r x")
-    apply (frule_tac p = p and v = v in  ptable_lift_preserved' [rotated] ; clarsimp)
-   apply clarsimp
+    apply (rule rewrite_or)
+    apply (case_tac "ptable_trace' h r x = {}")
+     apply (clarsimp simp: is_fault_pt_trace)
+    apply (frule_tac p = p and v = v in  pt_walk_preserved' [rotated] ; clarsimp)
+   apply (rule , simp)
    apply (erule disjE)
-    apply (clarsimp simp: ptrace_invalid_ptable_lift_none)
-   apply (clarsimp simp: ptrace_invalid_ptable_lift_none)
-  apply clarsimp
+    apply (clarsimp simp: ptrace_invalid_pt_walk_is_fault)
+   apply (clarsimp simp: ptrace_invalid_pt_walk_is_fault)
   apply (case_tac "p \<notin> ptable_trace' h r x")
-   apply (clarsimp simp: ptable_lift'_def lookup_pde'_def)
-   apply (clarsimp split: option.splits)
-    apply (case_tac x2 ; clarsimp)
-     apply (case_tac "ptable_trace' h r x = {}")
-      apply clarsimp
-      apply (clarsimp simp: ptable_trace'_def Let_def split:option.splits)
-       apply (clarsimp simp: get_pde'_def)
-      apply (clarsimp simp: get_pde'_def)
-     apply (clarsimp simp: ptable_trace_get_pde)
-    apply (clarsimp simp: ptable_trace_get_pde)
-   apply (case_tac x2 ; clarsimp)
-     apply (clarsimp simp: ptable_trace_get_pde)
-    apply (clarsimp simp: ptable_trace_get_pde)
-   apply (clarsimp simp: ptable_trace_get_pde)
-   apply (clarsimp simp: ptable_trace_lookup_pte)
-  apply clarsimp
-  apply (erule_tac disjE)
-   apply (clarsimp simp: ptable_trace'_def Let_def split:option.splits)
-   apply (clarsimp simp: ptable_lift'_def lookup_pde'_def get_pde'_def)
-   apply (case_tac x2 ; clarsimp)
-    apply (erule disjE)
-     apply (clarsimp simp: lookup_pte'_def get_pte'_def decode_heap_pte'_def decode_pde_def decode_pte_def decode_pte_small_def
-                     decode_pde_pt_def  decode_pde_section_def Let_def split:split_if_asm)
-     apply word_bitwise apply force
-    apply (clarsimp simp: decode_heap_pde'_def)
-   apply (clarsimp simp: decode_heap_pde'_def)
-  apply (clarsimp simp: ptable_trace'_def Let_def split:option.splits)
-  apply (clarsimp simp: ptable_lift'_def lookup_pde'_def get_pde'_def)
-  apply (case_tac x2 ; clarsimp)
-   apply (erule disjE)
-    apply (clarsimp simp: lookup_pte'_def get_pte'_def decode_heap_pte'_def  decode_pte_def)
-   apply (clarsimp simp: decode_heap_pde'_def decode_pde_def decode_pte_def decode_pte_small_def
-         decode_pde_pt_def  decode_pde_section_def Let_def split:split_if_asm)
-  apply (clarsimp simp: decode_pte_small_def)
-done
+   apply clarsimp
+   apply (frule_tac a = a and v = v in pt_walk_preserved' ; clarsimp)
+  apply (rule, simp)
+  apply (clarsimp simp: ptrace_invalid_pt_walk_is_fault)
+ done
 
 
 
-lemma  kernel_map_invariant: 
+lemma  kernel_map_invariant:
   "\<Turnstile> \<lbrace> \<lambda>s. kernel_state s \<and> aval lval s = Some vp \<and> aval rval s = Some v \<and> vp \<in> SM \<and> SM = kernel_safe_region' s \<and>
-             assigned_asids_consistent (root_map s) (incon_set s)  \<and> 
+             assigned_asids_consistent (root_map s) (incon_set s)  \<and>
             (Addr vp r- global_offset) \<in> \<Union>(ptable_trace' (heap s) (root s) ` UNIV) \<and>
-                 ((heap s) (Addr vp r- global_offset)) = Some w \<and> 
-                (decode_pde w = InvalidPDE \<or> decode_pte_small w = InvalidPTE) \<and>  
+                 ((heap s) (Addr vp r- global_offset)) = Some w \<and>
+                (decode_pde w = InvalidPDE \<or> decode_pte_small w = InvalidPTE) \<and>
                (\<exists>p pbits. decode_pde v = SectionPDE p pbits \<or> decode_pte_small v = SmallPagePTE p pbits) \<rbrace>
-                          lval ::= rval 
+                          lval ::= rval
                   \<lbrace>\<lambda>s. {asid s} \<times> UNIV \<inter> incon_set s = {} \<rbrace>"
-  apply_trace (vcg vcg:  assign_sound)
+  apply (vcgm vcg:  assign_sound)
   apply (rule conjI)
    apply (clarsimp simp: assigned_asids_consistent_def assigned_asid_va_map_def ran_def kernel_state_def)
    apply fastforce
-  apply (subgoal_tac "pde_comp (asid s) (heap s) (heap s(Addr (vp - global_offset) \<mapsto> v)) (root s) = {}")
+  apply (subgoal_tac "pde_comp' (asid s) (heap s) (heap s(Addr (vp - global_offset) \<mapsto> v)) (root s) = {}")
    apply clarsimp
    apply (clarsimp simp: asid_assumption_def assigned_asids_consistent_def assigned_asid_va_map_def ran_def kernel_state_def)
    apply fastforce
@@ -574,19 +607,19 @@ lemma  kernel_map_invariant:
 
 
 
-lemma  kernel_map_invariant': 
+lemma  kernel_map_invariant':
   "\<Turnstile> \<lbrace> \<lambda>s. kernel_state s \<and> aval lval s = Some vp \<and> aval rval s = Some v \<and> vp \<in> SM \<and> SM = kernel_safe_region' s \<and>
-         assigned_asids_consistent (root_map s) (incon_set s)  \<and> 
-            (Addr vp r- global_offset) \<in> \<Union>(ptable_trace' (heap s) (root s) ` UNIV) \<and> ((heap s) (Addr vp r- global_offset)) = Some w \<and> 
-                (decode_pde w = InvalidPDE \<or> decode_pte_small w = InvalidPTE) \<and>  
+         assigned_asids_consistent (root_map s) (incon_set s)  \<and>
+            (Addr vp r- global_offset) \<in> \<Union>(ptable_trace' (heap s) (root s) ` UNIV) \<and> ((heap s) (Addr vp r- global_offset)) = Some w \<and>
+                (decode_pde w = InvalidPDE \<or> decode_pte_small w = InvalidPTE) \<and>
                (\<exists>p pbits. decode_pde v = SectionPDE p pbits \<or> decode_pte_small v = SmallPagePTE p pbits) \<rbrace>
-                          lval ::= rval 
+                          lval ::= rval
                   \<lbrace>\<lambda>s. assigned_asids_consistent (root_map s) (incon_set s) \<rbrace>"
-  apply_trace (vcg vcg:  assign_sound)
+  apply (vcgm vcg:  assign_sound)
   apply (rule conjI)
    apply (clarsimp simp: assigned_asids_consistent_def assigned_asid_va_map_def ran_def kernel_state_def)
    apply fastforce
-  apply (subgoal_tac "pde_comp (asid s) (heap s) (heap s(Addr (vp - global_offset) \<mapsto> v)) (root s) = {}")
+  apply (subgoal_tac "pde_comp' (asid s) (heap s) (heap s(Addr (vp - global_offset) \<mapsto> v)) (root s) = {}")
    prefer 2
    apply (clarsimp simp: map_pde_comp_empty)
   by clarsimp
@@ -598,19 +631,19 @@ lemma  kernel_map_invariant':
 
 (* do this along with the ptable and pttrace etc  *)
 
-(* might have to see the multilevel page table assigning, or rampping*) 
+(* might have to see the multilevel page table assigning, or rampping*)
 
 
 (*  does kernel remaps the pages of the inactive processes (or inactive asids) *)
 
-lemma  
+lemma
   "\<Turnstile> \<lbrace> \<lambda>s. kernel_state s \<and> aval lval s = Some vp \<and> aval rval s = Some v \<and> vp \<in> SM \<and> SM = kernel_safe_region' s \<and>
          assigned_asids_consistent (root_map s) (incon_set s)  \<and>  rt \<in> root_log s \<and> rt \<noteq> root s \<and>
-            (Addr vp r- global_offset) \<in> \<Union>(ptable_trace' (heap s) rt ` UNIV) \<and> ((heap s) (Addr vp r- global_offset)) = Some w \<and> (decode_pde w = InvalidPDE \<or> decode_pte_small w = InvalidPTE) \<and>  
+            (Addr vp r- global_offset) \<in> \<Union>(ptable_trace' (heap s) rt ` UNIV) \<and> ((heap s) (Addr vp r- global_offset)) = Some w \<and> (decode_pde w = InvalidPDE \<or> decode_pte_small w = InvalidPTE) \<and>
                (\<exists>p pbits. decode_pde v = SectionPDE p pbits \<or> decode_pte_small v = SmallPagePTE p pbits) \<rbrace>
-                             lval ::= rval 
+                             lval ::= rval
                   \<lbrace>\<lambda>s. some_invariant \<rbrace>"
- 
+
 oops
 
 
@@ -622,14 +655,14 @@ find_theorems "Flush (flushASID _)"
 
 lemma  remap_section_entry_current_page_table:
   "\<Turnstile> \<lbrace> \<lambda>s. kernel_state s \<and> aval lval s = Some vp \<and> aval rval s = Some v \<and> vp \<in> SM \<and> SM = kernel_safe_region' s \<and>
-             assigned_asids_consistent (root_map s) (incon_set s)  \<and> 
-             (Addr vp r- global_offset) \<in> \<Union>(ptable_trace' (heap s) (root s) ` UNIV) \<and> 
-                ((heap s) (Addr vp r- global_offset)) = Some w \<and> (\<exists>p pbits. decode_pde w = SectionPDE p pbits) \<and>  
+             assigned_asids_consistent (root_map s) (incon_set s)  \<and>
+             (Addr vp r- global_offset) \<in> \<Union>(ptable_trace' (heap s) (root s) ` UNIV) \<and>
+                ((heap s) (Addr vp r- global_offset)) = Some w \<and> (\<exists>p pbits. decode_pde w = SectionPDE p pbits) \<and>
                    (\<exists>p pbits. decode_pde v = SectionPDE p pbits) \<and> asid s = a \<rbrace>
                           lval ::= rval ;; Flush (flushASID a)
                   \<lbrace>\<lambda>s. {asid s} \<times> UNIV \<inter> incon_set s = {} \<rbrace>"
 (* simple to prove in case of asid flush, it should be va flush *)
-  apply_trace (vcg vcg:  assign_sound)
+  apply (vcgm vcg:  assign_sound)
   apply (rule conjI)
    apply (clarsimp simp: assigned_asids_consistent_def assigned_asid_va_map_def ran_def kernel_state_def)
    apply fastforce
@@ -641,18 +674,18 @@ lemma  remap_section_entry_current_page_table:
 lemma remap_section_entry_inactive_page_table:
   "\<Turnstile> \<lbrace> \<lambda>s. kernel_state s \<and> aval lval s = Some vp \<and> aval rval s = Some v \<and> vp \<in> SM \<and> SM = kernel_safe_region' s \<and>
          assigned_asids_consistent (root_map s) (incon_set s)  \<and> rt \<in> root_log s \<and> rt \<noteq> root s \<and>  (* remove this condition later *)
-                  (Addr vp r- global_offset) \<in> \<Union>(ptable_trace' (heap s) rt ` UNIV) \<and> ((heap s) (Addr vp r- global_offset)) = Some w \<and> (\<exists>p pbits. decode_pde w = SectionPDE p pbits) \<and>  
+                  (Addr vp r- global_offset) \<in> \<Union>(ptable_trace' (heap s) rt ` UNIV) \<and> ((heap s) (Addr vp r- global_offset)) = Some w \<and> (\<exists>p pbits. decode_pde w = SectionPDE p pbits) \<and>
                    (\<exists>p pbits. decode_pde v = SectionPDE p pbits) \<and> root_map s rt = Some a \<rbrace>
                      lval ::= rval ;; Flush (flushASID a)
                   \<lbrace>\<lambda>s. assigned_asids_consistent (root_map s) (incon_set s) \<rbrace>"
    (* do it with kernel_writing_to_inactive_process_page_table_and_flush *)
-  apply_trace (vcg vcg:  assign_sound)
+  apply (vcgm vcg:  assign_sound)
   apply (rule conjI)
    apply (clarsimp simp: assigned_asids_consistent_def  assigned_asid_va_map_def ran_def kernel_state_def)
    apply auto [1]
   apply (rule conjI)
    apply (clarsimp simp: kernel_state_def)
-  apply (subgoal_tac "pde_comp (asid s) (heap s) (heap s(Addr (vp - global_offset) \<mapsto> v)) (root s) = {}")
+  apply (subgoal_tac "pde_comp' (asid s) (heap s) (heap s(Addr (vp - global_offset) \<mapsto> v)) (root s) = {}")
    apply clarsimp
    apply (clarsimp simp: assigned_asids_consistent_def)
    apply force
@@ -665,13 +698,13 @@ lemma remap_section_entry_inactive_page_table:
 
 lemma  remap_scond_level_entry_inactive_page_table:   (* not relevant to entries as we are flushing asid, will be relevant if we flush vadder set *)
   "\<Turnstile> \<lbrace> \<lambda>s. kernel_state s \<and> aval lval s = Some vp \<and> aval rval s = Some v \<and> vp \<in> SM \<and> SM = kernel_safe_region' s \<and>
-             assigned_asids_consistent (root_map s) (incon_set s)  \<and> 
-             (Addr vp r- global_offset) \<in> \<Union>(ptable_trace' (heap s) (root s) ` UNIV) \<and> 
-                ((heap s) (Addr vp r- global_offset)) = Some w \<and> (\<exists>p pbits. decode_pte w = SmallPagePTE p pbits) \<and>  
+             assigned_asids_consistent (root_map s) (incon_set s)  \<and>
+             (Addr vp r- global_offset) \<in> \<Union>(ptable_trace' (heap s) (root s) ` UNIV) \<and>
+                ((heap s) (Addr vp r- global_offset)) = Some w \<and> (\<exists>p pbits. decode_pte w = SmallPagePTE p pbits) \<and>
                    (\<exists>p pbits. decode_pte v = SmallPagePTE p pbits) \<and> asid s = a \<rbrace>
                           lval ::= rval ;; Flush (flushASID a)
                   \<lbrace>\<lambda>s. {asid s} \<times> UNIV \<inter> incon_set s = {} \<rbrace>"
- apply_trace (vcg vcg:  assign_sound)
+ apply (vcgm vcg:  assign_sound)
   apply (rule conjI)
    apply (clarsimp simp: assigned_asids_consistent_def assigned_asid_va_map_def ran_def kernel_state_def)
    apply fastforce
@@ -683,18 +716,18 @@ lemma  remap_scond_level_entry_inactive_page_table:   (* not relevant to entries
 lemma remap_second_level_entry_inactive_page_table:
   "\<Turnstile> \<lbrace> \<lambda>s. kernel_state s \<and> aval lval s = Some vp \<and> aval rval s = Some v \<and> vp \<in> SM \<and> SM = kernel_safe_region' s \<and>
          assigned_asids_consistent (root_map s) (incon_set s)  \<and> rt \<in> root_log s \<and> rt \<noteq> root s \<and>  (* remove this condition later *)
-                  (Addr vp r- global_offset) \<in> \<Union>(ptable_trace' (heap s) rt ` UNIV) \<and> ((heap s) (Addr vp r- global_offset)) = Some w \<and> (\<exists>p pbits. decode_pte w = SmallPagePTE p pbits) \<and>  
+                  (Addr vp r- global_offset) \<in> \<Union>(ptable_trace' (heap s) rt ` UNIV) \<and> ((heap s) (Addr vp r- global_offset)) = Some w \<and> (\<exists>p pbits. decode_pte w = SmallPagePTE p pbits) \<and>
                    (\<exists>p pbits. decode_pte v = SmallPagePTE p pbits) \<and> root_map s rt = Some a \<rbrace>
                      lval ::= rval ;; Flush (flushASID a)
                   \<lbrace>\<lambda>s. assigned_asids_consistent (root_map s) (incon_set s) \<rbrace>"
   (* same proof as remap_section_entry_inactive_page_table *)
-  apply_trace (vcg vcg:  assign_sound)
+  apply (vcgm vcg:  assign_sound)
   apply (rule conjI)
    apply (clarsimp simp: assigned_asids_consistent_def  assigned_asid_va_map_def ran_def kernel_state_def)
    apply auto [1]
   apply (rule conjI)
    apply (clarsimp simp: kernel_state_def)
-  apply (subgoal_tac "pde_comp (asid s) (heap s) (heap s(Addr (vp - global_offset) \<mapsto> v)) (root s) = {}")
+  apply (subgoal_tac "pde_comp' (asid s) (heap s) (heap s(Addr (vp - global_offset) \<mapsto> v)) (root s) = {}")
    apply clarsimp
    apply (clarsimp simp: assigned_asids_consistent_def)
    apply force
@@ -708,278 +741,20 @@ lemma remap_second_level_entry_inactive_page_table:
 thm get_pte'_def
 
 
-lemma 
+lemma
   "\<Turnstile> \<lbrace> \<lambda>s. kernel_state s \<and> aval lval s = Some vp \<and> aval rval s = Some v \<and> vp \<in> SM \<and> SM = kernel_safe_region' s \<and>
-             assinged_asids_consistent (root_map s) (incon_set s)  \<and> 
-             (Addr vp r- global_offset) \<in> \<Union>(ptable_trace' (heap s) (root s) ` UNIV) \<and> 
-                ((heap s) (Addr vp r- global_offset)) = Some w \<and>  
-            (\<exists>p. decode_pde w = PageTablePDE p \<and>  (\<exists>w p1 pbits. (heap s) (p r+ ((vaddr_pt_index  vp) << 2))  = Some w \<and>  decode_pte w  = SmallPagePTE p1 pbits)) \<and>  
+             assigned_asids_consistent (root_map s) (incon_set s)  \<and>
+             (Addr vp r- global_offset) \<in> \<Union>(ptable_trace' (heap s) (root s) ` UNIV) \<and>
+                ((heap s) (Addr vp r- global_offset)) = Some w \<and>
+            (\<exists>p. decode_pde w = PageTablePDE p \<and>  (\<exists>w p1 pbits. (heap s) (p r+ ((vaddr_pt_index  vp) << 2))  = Some w \<and>  decode_pte w  = SmallPagePTE p1 pbits)) \<and>
                    (\<exists>p pbits. decode_pde v = SectionPDE p pbits) \<and> asid s = a \<rbrace>
                           lval ::= rval ;; Flush (flushASID a)
-                  \<lbrace>\<lambda>s. (asid_va_set (asid s)) \<inter> incon_set s = {} \<rbrace>"
-  
+                  \<lbrace>\<lambda>s. {asid s} \<times> UNIV \<inter> incon_set s = {} \<rbrace>"
+
 (*  *)
 
 
 oops
-
-(* have a review *)
-
-lemma 
-  "\<Turnstile> \<lbrace> \<lambda>s. kernel_state s \<and> aval lval s = Some vp \<and> aval rval s = Some v \<and> vp \<in> SM \<and> SM = kernel_safe_region' s \<and>
-      assinged_asids_consistent (root_map s) (incon_set s)  \<and>  Addr vp \<in> ptable_mapped' (heap s) (root s) \<and>
-               (\<exists>p p_bits. get_pde' (heap s) (root s) (Addr vp) = Some (SectionPDE p p_bits) \<and> V = vspace_section_entry (heap s) (root s) (SectionPDE p p_bits) ) \<rbrace>
-                     lval ::= rval ;; Flush (flushvarange V) ;; SetMode User
-                  \<lbrace>\<lambda>s. safe_set (SM_user (heap s) (root s)) s \<and>  heap s (Addr vp r- global_offset) = Some v\<rbrace>"
-  apply_trace (vcg vcg: weak_pre_write [of SM])
-  apply (rule conjI)
-   apply (clarsimp simp: safe_set_def safe_memory_def ptrace_set_def)
-  apply (rule conjI)
-   apply (clarsimp simp: kernel_state_def)
-  apply (clarsimp simp: safe_set_def)
-  apply (rule conjI)
-   apply (clarsimp simp: safe_memory_def SM_user_def ptrace_set_def)
-  apply (clarsimp simp: con_set_def)
-  apply (rule conjI)
-   apply (clarsimp simp: kernel_state_def assinged_asids_consistent_def asids_va_set_def set_of_assigned_asids_def asid_va_set_def)
-   apply force
-  apply (subgoal_tac "ptable_lift' (heap s) (root s) (Addr va) = ptable_lift' (heap s(Addr (vp - global_offset) \<mapsto> v)) (root s) (Addr va)")
-   apply (clarsimp simp: )
-
-oops
-   
-
-
-definition 
-   pd_idx_offset :: "32 word \<Rightarrow> machine_word"
-where
-  "pd_idx_offset vp = ((vaddr_pd_index vp) << 2)"
-
-
-definition
-  va_to_pa_offset :: "vaddr \<Rightarrow> 32 word \<Rightarrow> vaddr set \<rightharpoonup> paddr"
-where
-  "va_to_pa_offset va offset S \<equiv> if va \<in> S then Some (Addr (addr_val(va r+ offset))) else None"
-
-
-
-definition
-  st_initial :: "p_state \<Rightarrow> bool"
-where
-  "st_initial s   \<equiv>   heap s (root s) = Some 0x00000002 \<and> heap s (root s r+ 0x4) = Some 0x00100002 \<and> 
-                           heap s (root s r+ 0x8) = Some 0x00000C01 \<and>  heap s (root s r+ 0x00000C00) = Some 0x0000F032 \<and>
-                           root s = Addr 0 \<and>  mode s = Kernel  \<and> asid s = 0 \<and> root_map s (Addr 0) = Some 0 \<and> partial_inj (root_map s)"
-
-
-
-definition
-  vspace_section :: "32 word set"
-where
-  "vspace_section \<equiv> {va. (pd_idx_offset va = 0 \<or>  pd_idx_offset va = 4 )  }"
-
-
-definition
-  vadd_entries :: "32 word set"
-where
-  "vadd_entries \<equiv> {0x00000000 , 0x00000004}"
-
-
-definition 
-  kernel_memory :: "32 word set"
-where
-  "kernel_memory  = vspace_section - vadd_entries"
-
-
-
-definition
-  vas_user_mappings :: "32 word set"
-where
-  "vas_user_mappings  \<equiv> {va. pd_idx_offset va = 0x8 \<and> 0xC00 + ((va >> 12) && 0xFF << 2) = 0x00000C00} - {0x00000000 , 0x00000004 , 0x00000008 , 0x00000C00}"
-
-
-lemma aval_state_heap_mode_eq[simp]:
-  "(aval e (s\<lparr> mode := m, heap := h\<rparr>) = Some v) = (aval e (s\<lparr>heap := h\<rparr>) = Some v)"
-  by (induct e arbitrary: v; clarsimp split: option.splits; fastforce)
-            
-
-
-lemma  [simp]:
-  "st_initial s \<Longrightarrow> mode s = Kernel"
-  by (clarsimp simp: st_initial_def)
-
-
-lemma  user_ptrace:
-  "\<lbrakk>st_initial s;  va \<in> vas_user_mappings\<rbrakk>
-              \<Longrightarrow> ptable_trace' (heap s) (root s) (Addr va) = {Addr 8, Addr 0xC00}"
-  apply (clarsimp simp: vaddr_offset_def mask_def vas_user_mappings_def pd_idx_offset_def vaddr_pd_index_def ptable_trace'_def Let_def decode_heap_pde'_def st_initial_def decode_pde_def decode_pde_pt_def
-                           pt_base_mask_def vaddr_pt_index_def)
-  by blast
-
-lemma [simp]:
-  "ptrace_set V (s\<lparr>incon_set := is, mode := m\<rparr>) = ptrace_set V s"
-  by (clarsimp simp: ptrace_set_def)
-
-
-lemma user_ptable_lift_defined:
-  "\<lbrakk>st_initial s;  va \<in> vas_user_mappings\<rbrakk>  \<Longrightarrow> ptable_lift_m (heap s) (root s) User (Addr va) = Some ((Addr 0xF000) r+ vaddr_offset ArmSmallPage va)"
-  apply (clarsimp simp: vas_user_mappings_def ptable_lift_m_def lookup_pde_perm_def filter_pde_def lookup_pde'_def get_pde'_def vaddr_pd_index_def pd_idx_offset_def)
-  apply (clarsimp simp: decode_heap_pde'_def st_initial_def)
-  apply (clarsimp simp: decode_pde_def decode_pde_pt_def  lookup_pte'_def get_pte'_def pt_base_mask_def decode_heap_pte'_def vaddr_pt_index_def mask_def)
-  apply (clarsimp simp: decode_pte_def decode_pte_small_def user_perms_def perm_bits_pte_small_def addr_base_def mask_def)
-done
-
-
-lemma  vas_user_mappings_ptace:
-  "\<lbrakk>st_initial s; vp1 \<in> vas_user_mappings;  vp2 \<in> vas_user_mappings\<rbrakk>
-         \<Longrightarrow> Addr (0xF000 + vaddr_offset ArmSmallPage vp1) \<notin> ptable_trace' (heap s) (root s) (Addr vp2)"
-  apply (frule_tac va = vp2 in  user_ptrace; clarsimp simp: vaddr_offset_def mask_def)
-  by word_bitwise
-
-
-           
-lemma ptable_lift_preserved_m':
-  "\<lbrakk>ptable_lift_m h r m vp = Some pa; p \<notin> ptable_trace' h r vp\<rbrakk> \<Longrightarrow> ptable_lift_m (h(p \<mapsto> v)) r m vp = Some pa"
- by (clarsimp simp: ptable_lift_preserved_m)
-
-lemma [simp]:
-  "st_initial s \<Longrightarrow> (asid s ,va ) \<in> asids_va_set (root_map s)"
-  apply (clarsimp simp: st_initial_def asids_va_set_def set_of_assigned_asids_def asid_va_set_def) by force
-
-
-lemma [simp]:
-  "(asid s ,va ) \<in> asids_va_set (root_map s) \<and> asids_va_set (root_map s) \<inter> incon_set s = {} \<Longrightarrow> (asid s, va) \<notin> incon_set s"
-  apply (clarsimp simp: asids_va_set_def set_of_assigned_asids_def asid_va_set_def) by force
-
-
-lemma st_initial_user_safe_set [simp]:
-  "\<lbrakk>st_initial s ; assinged_asids_consistent (root_map s) (incon_set s) \<rbrakk> \<Longrightarrow> 
-                   safe_set vas_user_mappings (s\<lparr>mode := User\<rparr>)"
-  apply (clarsimp simp: safe_set_def con_set_def safe_memory_def assinged_asids_consistent_def)
-  apply (frule_tac va = va in user_ptable_lift_defined; clarsimp simp: ptrace_set_def user_ptrace vaddr_offset_def mask_def)
-  by word_bitwise
- 
-(*  safe set established after changing the mode  *)
-
-lemma assignments_safe_kernel_user:
-  "\<Turnstile> \<lbrace> \<lambda>s. st_initial s \<and> aval lval1 s = Some vp1 \<and> aval rval1 s = Some v1 \<and> vp1 \<in> vas_user_mappings \<and> 
-            aval lval2 (s\<lparr>heap := heap s(Addr 0xF000 r+ vaddr_offset ArmSmallPage vp1 \<mapsto> v1)\<rparr>) = Some vp2 \<and> 
-            aval rval2 (s\<lparr>heap := heap s(Addr 0xF000 r+ vaddr_offset ArmSmallPage vp1 \<mapsto> v1)\<rparr>) = Some v2 \<and> vp2 \<in> vas_user_mappings  \<and>
-                 assinged_asids_consistent (root_map s) (incon_set s)\<rbrace>  
-               SetMode User ;; lval1 ::= rval1 ;; lval2 ::= rval2 
-            \<lbrace>\<lambda>s. safe_set vas_user_mappings s \<and> heap s (Addr 0xF000 r+ vaddr_offset ArmSmallPage vp2) = Some v2\<rbrace>"
-  apply_trace (vcg vcg: weak_pre_write')
-   (* clarsimp is giving me problems *)
-  apply (frule_tac va = vp1 in user_ptable_lift_defined ; clarsimp)
-  apply (frule_tac va = vp2 in user_ptable_lift_defined ; clarsimp)
-  by (frule_tac p = "Addr (0xF000 + vaddr_offset ArmSmallPage vp1)" and vp = "Addr vp2"  and v = v1 in  ptable_lift_preserved_m' ; clarsimp simp: vas_user_mappings_ptace)
-
-
-lemma [simp]:
-  "con_set vas_user_mappings (s\<lparr>mode := User\<rparr>) =  con_set vas_user_mappings s"
-  by (clarsimp simp: con_set_def)
-
-
-
-(* kernel is writing to the pagetable, and then changing the mode, it requires flushing *)
-(* this can be proved, but also i should make difference of the mapping of the page table and removing/or remapping, I should have a different memory model, in which all of the vas are mapped, either to invalid or to a valid page-table *)
-
-lemma  [simp]:
-  "st_initial s \<Longrightarrow> asid s \<in> set_of_assigned_asids (root_map s)"
-  apply (clarsimp simp: st_initial_def set_of_assigned_asids_def)
-  by force
-
-lemma [simp]:
-  "\<lbrakk>st_initial s; assinged_asids_consistent (root_map s) (incon_set s)\<rbrakk> \<Longrightarrow> con_set kernel_memory s"
-  apply (clarsimp simp: assinged_asids_consistent_def con_set_def asids_va_set_def set_of_assigned_asids_def asid_va_set_def st_initial_def)
-  apply force
-done
-
-
-lemma state_intitial_ptable_lift_offset':
-  "\<lbrakk>st_initial s \<rbrakk> \<Longrightarrow>
-        \<forall>va\<in>vspace_section.  ptable_lift_m (heap s) (root s) (mode s) (Addr va) = va_to_pa_offset (Addr va) 0 (Addr `vspace_section)"
-  apply (clarsimp simp: st_initial_def vspace_section_def va_to_pa_offset_def ptable_lift_m_def lookup_pde'_def get_pde'_def decode_heap_pde'_def vaddr_pd_index_def pd_idx_offset_def
-                decode_pde_def decode_pde_section_def addr_base_def vaddr_offset_def mask_def)
-   by word_bitwise
-  
-
-lemma state_intitial_ptable_lift_offset2':
-  "\<lbrakk>st_initial s \<rbrakk> \<Longrightarrow>
-        \<forall>va\<in>kernel_memory.  ptable_lift' (heap s) (root s) (Addr va) = va_to_pa_offset (Addr va) 0 (Addr `vspace_section)"
-  using state_intitial_ptable_lift_offset' by (clarsimp simp: kernel_memory_def)
- 
-
-lemma kernel_memory_vspace:
-  "vp : kernel_memory \<Longrightarrow> vp : vspace_section"
-  by (simp add: kernel_memory_def)
-
-lemma va_to_pa_offset_0 [simp]:
-  "vp : kernel_memory \<Longrightarrow> va_to_pa_offset (Addr vp) 0 (Addr ` vspace_section) = Some (Addr vp)"
-  by (simp add: va_to_pa_offset_def kernel_memory_vspace)
-
-lemma state_intial_element_ptrace [simp]:
-  "\<lbrakk>st_initial s;  va \<in> kernel_memory \<rbrakk> \<Longrightarrow>  Addr va \<notin> ptrace_set kernel_memory s"
-  apply (clarsimp simp: st_initial_def ptrace_set_def kernel_memory_def vspace_section_def)
-  apply (erule_tac P = "pd_idx_offset a = 0" in disjE)
-   apply (subgoal_tac "ptable_trace' (heap s) (Addr 0) (Addr a) = {Addr 0}")
-    using vadd_entries_def  apply force
-   apply (clarsimp simp: ptable_trace'_def Let_def pd_idx_offset_def decode_heap_pde'_def
-              decode_pde_def decode_pde_section_def)
-  apply (subgoal_tac "ptable_trace' (heap s) (Addr 0) (Addr a) = {Addr 4}")
-   using vadd_entries_def  apply force
-  by (clarsimp simp: ptable_trace'_def Let_def pd_idx_offset_def decode_heap_pde'_def
-                decode_pde_def decode_pde_section_def)
-
-
-
-lemma kernel_write_outside_mode_switch:
-  "\<Turnstile> \<lbrace> \<lambda>s. st_initial s \<and> aval lval s = Some vp \<and> aval rval s = Some v \<and> 
-     vp \<in> kernel_memory \<and>  vp \<in> kernel_memory \<and> vp \<notin> {0x00000008 , 0x00000C00} \<and>
-                 assinged_asids_consistent (root_map s) (incon_set s)\<rbrace>  
-                            lval ::= rval  ;; SetMode User 
-            \<lbrace>\<lambda>s. safe_set vas_user_mappings s \<rbrace>"
- apply_trace (vcg vcg: weak_pre_write [of kernel_memory])
-  apply rule
-  apply (clarsimp simp: safe_set_def safe_memory_def state_intitial_ptable_lift_offset2')
-  apply (subgoal_tac "ptable_lift' (heap s) (root s) (Addr vp) = va_to_pa_offset (Addr vp) 0 (Addr `vspace_section)")
-  prefer 2
-   using state_intitial_ptable_lift_offset' apply (clarsimp simp: kernel_memory_def)
-   apply clarsimp
-  apply (clarsimp simp: safe_set_def)
-  apply rule
-   prefer 2
-  apply (clarsimp simp: con_set_def)
-   apply (rule)
-    apply (clarsimp simp: assinged_asids_consistent_def)
-    apply (clarsimp simp: pde_comp_def )
-   find_theorems "lookup_pde'"
- (* can be done  *)
-
-sorry
-
- 
-(* writing to a valid page table entry, flush requires *)
-
-lemma 
-  "\<Turnstile> \<lbrace> \<lambda>s. st_initial s \<and> aval lval s = Some vp \<and> aval rval s = Some v \<and> vp \<in> kernel_memory \<and>  vp \<in> kernel_memory \<and> vp \<in> {0x00000008 , 0x00000C00} \<and>
-                 assinged_asids_consistent (root_map s) (incon_set s) \<and> (asid s) = a\<rbrace>  
-                            lval ::= rval ;; Flush (flushASID a) ;; SetMode User 
-                     \<lbrace>\<lambda>s. safe_set vas_user_mappings s \<rbrace>"
- apply_trace (vcg vcg: weak_pre_write [of kernel_memory])
-  apply rule
-  apply (clarsimp simp: safe_set_def safe_memory_def state_intitial_ptable_lift_offset2')
-  apply (subgoal_tac "ptable_lift' (heap s) (root s) (Addr vp) = va_to_pa_offset (Addr vp) 0 (Addr `vspace_section)")
-  prefer 2
-   using state_intitial_ptable_lift_offset' apply (clarsimp simp: kernel_memory_def)
-   apply clarsimp
-  apply (clarsimp simp: safe_set_def)
-  apply rule
-   prefer 2
-  apply (clarsimp simp: con_set_def)
- (* can be done  *)
-
-sorry
-
 
 
 
@@ -994,6 +769,3 @@ sorry
 
 
 end
-
-
-
