logic/Safe_Set.thy
@@ -28,33 +28,40 @@ where
   "safe_set V s \<equiv>  (safe_memory V s \<and> con_set V s)"
  
 
-
 lemma cons_set_preserved:
   "\<lbrakk> \<forall>va\<in>SM. \<exists>p.  ptable_lift_m (heap s) (root s) (mode s) (Addr va) = Some p \<and> p \<notin> ptrace_set SM s;
           \<forall>va\<in>SM. (asid s, va) \<notin> incon_set s; p \<notin> ptrace_set SM s; va \<in> SM\<rbrakk>  \<Longrightarrow> 
-              (asid s, va) \<notin> pde_comp (asid s) (heap s) (heap s(p \<mapsto> v)) (root s)"
+              (asid s, va) \<notin> pde_comp' (asid s) (heap s) (heap s(p \<mapsto> v)) (root s)"
   apply (case_tac "mode s")
    apply (drule_tac x = va in bspec ; clarsimp)
    apply (drule_tac x = va in bspec , simp)
-   apply (clarsimp simp: pde_comp_def ptable_lift'_def ptrace_set_def)
+   apply (clarsimp simp: pde_comp'_def pt_walk_def is_fault_def ptrace_set_def)
    apply (drule_tac x = va in bspec , simp)
-   apply (clarsimp simp: ptable_trace'_def  Let_def lookup_pde'_def  get_pde'_def decode_heap_pde'_def split: option.splits pde.splits)
+   apply (clarsimp simp: ptable_trace'_def  Let_def lookup_pde'_def  get_pde'_def decode_heap_pde'_def split: option.splits pde.splits pte.splits)
+     apply (frule_tac x = "addr_val x" in bspec , simp)
+     apply (clarsimp simp: lookup_pte'_def get_pte'_def decode_heap_pte'_def split:option.splits pte.splits)
+    apply (frule_tac x = "addr_val x" in bspec , simp)
+    apply (clarsimp simp: lookup_pte'_def get_pte'_def decode_heap_pte'_def split:option.splits pte.splits)
    apply (frule_tac x = "addr_val x" in bspec , simp)
    apply (clarsimp simp: lookup_pte'_def get_pte'_def decode_heap_pte'_def split:option.splits pte.splits)
   apply (drule_tac x = va in bspec ; clarsimp)
   apply (frule ptable_lift_m_user)
   apply (drule_tac x = va in bspec , simp)
-  apply (clarsimp simp: pde_comp_def ptable_lift'_def ptrace_set_def)
+  apply (clarsimp simp: pde_comp'_def pt_walk_def is_fault_def ptrace_set_def)
   apply (drule_tac x = va in bspec , simp)
-  apply (clarsimp simp: ptable_trace'_def  Let_def lookup_pde'_def  get_pde'_def decode_heap_pde'_def split: option.splits pde.splits)
-  apply (drule_tac x = "addr_val x" in bspec , simp)
- apply (clarsimp simp: lookup_pte'_def get_pte'_def decode_heap_pte'_def split:option.splits pte.splits)
+  apply (clarsimp simp: ptable_trace'_def  Let_def lookup_pde'_def  get_pde'_def decode_heap_pde'_def split: option.splits pde.splits pte.splits)
+    apply (drule_tac x = "addr_val x" in bspec , simp)
+    apply (clarsimp simp: lookup_pte'_def get_pte'_def decode_heap_pte'_def split:option.splits pte.splits)
+   apply (frule_tac x = "addr_val x" in bspec , simp)
+   apply (clarsimp simp: lookup_pte'_def get_pte'_def decode_heap_pte'_def split:option.splits pte.splits)
+  apply (frule_tac x = "addr_val x" in bspec , simp)
+  apply (clarsimp simp: lookup_pte'_def get_pte'_def decode_heap_pte'_def split:option.splits pte.splits)
  done
 
 lemma safe_set_preserved:
   "\<Turnstile> \<lbrace> \<lambda>s. safe_set SM s \<and> (\<exists>vp v. aval lval s = Some vp \<and> aval rval s = Some v \<and> vp \<in> SM)\<rbrace>
                 lval ::= rval  \<lbrace>\<lambda>s. safe_set SM s \<rbrace>"
-  apply vcg
+  apply vcgm
   apply (rule conjI, clarsimp simp: safe_set_def  con_set_def)
   apply (clarsimp simp: safe_set_def safe_memory_def)
   apply (frule_tac x = vp in bspec ; safe)
@@ -83,9 +90,9 @@ lemma safe_set_preserved':
 lemma weak_pre_write:
   "\<Turnstile> \<lbrace> \<lambda>s. safe_set SM s \<and> (\<exists>vp v. aval lval s = Some vp \<and> aval rval s = Some v \<and> vp \<in> SM \<and> 
      Q (s \<lparr> heap := heap s (the (ptable_lift_m (heap s) (root s) (mode s) (Addr vp)) \<mapsto> v),
-             incon_set := incon_set s \<union> pde_comp (asid s) (heap s) (heap s(the (ptable_lift_m (heap s) (root s) (mode s) (Addr vp)) \<mapsto> v)) (root s)\<rparr>)) \<rbrace> 
+             incon_set := incon_set s \<union> pde_comp' (asid s) (heap s) (heap s(the (ptable_lift_m (heap s) (root s) (mode s) (Addr vp)) \<mapsto> v)) (root s)\<rparr>)) \<rbrace> 
            lval ::= rval  \<lbrace>Q\<rbrace>"
-  apply (vcg , clarsimp simp: safe_set_def safe_memory_def con_set_def)
+  apply (vcgm , clarsimp simp: safe_set_def safe_memory_def con_set_def)
   by fastforce
  
 
@@ -100,7 +107,8 @@ lemma hoare_post_conj:
 lemma weak_pre_write':
   "\<Turnstile> \<lbrace> \<lambda>s. safe_set SM s \<and> (\<exists>vp v. aval lval s = Some vp \<and> aval rval s = Some v \<and> vp \<in> SM \<and> 
      Q (s \<lparr>heap := heap s (the ( ptable_lift_m (heap s) (root s) (mode s) (Addr vp)) \<mapsto> v),
-             incon_set := incon_set s \<union> pde_comp (asid s) (heap s) (heap s(the (ptable_lift_m (heap s) (root s) (mode s) (Addr vp)) \<mapsto> v)) (root s)\<rparr>)) \<rbrace>
+             incon_set := incon_set s \<union> pde_comp' (asid s) (heap s) (heap s(the (ptable_lift_m (heap s)
+                           (root s) (mode s) (Addr vp)) \<mapsto> v)) (root s)\<rparr>)) \<rbrace>
              lval ::= rval  \<lbrace>\<lambda>s. safe_set SM s \<and> Q s \<rbrace>"
   by (rule hoare_post_conj, rule safe_set_preserved', rule weak_pre_write)
 
@@ -121,9 +129,9 @@ lemma weak_pre_write'_user:
   apply clarsimp
   apply (clarsimp simp: safe_set_def con_set_def safe_memory_def)
   apply (drule_tac x = vp in bspec; clarsimp)
-  apply (subgoal_tac "incon_set s = incon_set s \<union> pde_comp (asid s) (heap s) (heap s(the (ptable_lift_m (heap s) (root s) (mode s) (Addr vp)) \<mapsto> v)) (root s)")
+  apply (subgoal_tac "incon_set s = incon_set s \<union> pde_comp' (asid s) (heap s) (heap s(the (ptable_lift_m (heap s) (root s) (mode s) (Addr vp)) \<mapsto> v)) (root s)")
    apply (clarsimp simp: safe_set_def con_set_def safe_memory_def)
-  apply (subgoal_tac "pde_comp (asid s) (heap s) (heap s(the (ptable_lift_m (heap s) (root s) (mode s) (Addr vp)) \<mapsto> v)) (root s) = {}")
+  apply (subgoal_tac "pde_comp' (asid s) (heap s) (heap s(the (ptable_lift_m (heap s) (root s) (mode s) (Addr vp)) \<mapsto> v)) (root s) = {}")
    apply clarsimp
   apply (drule_tac x = vp in bspec , clarsimp)
   apply (clarsimp simp: ptable_mapped_def)
@@ -172,7 +180,7 @@ lemma  user_safe_set_established:
   "\<Turnstile> \<lbrace> \<lambda>s. \<exists>rt. aval ttbr0 s = Some rt \<and>  mode s = Kernel\<rbrace>  
                 UpdateTTBR0 ttbr0 ;; UpdateASID a ;;  Flush (flushASID a) ;;  SetMode User 
            \<lbrace>\<lambda>s. safe_set (SM_user (heap s) (root s)) s\<rbrace>"
-  apply vcg
+  apply vcgm
   by (clarsimp simp: safe_set_def con_set_def)
   
 lemma [simp]:
