logic/VCG_Check.thy
@@ -13,27 +13,66 @@ begin
 lemma  write_consistent_defined_address:
   "\<Turnstile> \<lbrace> \<lambda>s. aval lval s = Some vp \<and> aval rval s = Some v \<and> (asid s, vp) \<notin> incon_set s \<and>
       ptable_lift_m (heap s) (root s) (mode s) (Addr vp) = Some pp \<rbrace>  lval ::= rval \<lbrace>\<lambda>s. heap s pp = Some v \<rbrace>"
-   by vcg
+   by vcgm
  
 (* successful memory writes to inconsistent address after flushing, in Kernel Mode *) 
 
+(* new stuff *)
+lemma [simp]:
+  "mem_read_hp' (asid s) (incon_set s) (heap s) (root s) (Addr x2) = Some v
+                \<Longrightarrow> mem_read_hp' (asid s) {} (heap s) (root s) (Addr x2) = Some v"
+  apply (clarsimp simp: mem_read_hp'_def split: split_if_asm)
+done
+
+
+lemma [simp]:
+  "aval e s = Some v \<Longrightarrow> aval e (s\<lparr>incon_set := {}\<rparr>) = Some v "
+  by (induct e arbitrary: v; clarsimp split: option.splits; fastforce)
+
+(* new stuff *)
 lemma flush_TLB_mem_write:
   "\<Turnstile> \<lbrace> \<lambda>s. aval lval s = Some vp \<and> aval rval s = Some v \<and> (asid s, vp) \<in> incon_set s \<and>  mode s = Kernel \<and> 
       ptable_lift_m (heap s) (root s) (mode s) (Addr vp) = Some pp \<rbrace>  Flush flushTLB ;; lval ::= rval \<lbrace>\<lambda>s. heap s pp = Some v \<rbrace>"
-  by vcg
- 
+  by vcgm
 
+lemma[simp]:
+  "mem_read_hp' (asid s) (incon_set s) (heap s) (root s) (Addr x2) = Some v
+                \<Longrightarrow> mem_read_hp' (asid s) {av \<in> incon_set s. fst av \<noteq> asid s} (heap s) (root s) (Addr x2) = Some v"
+  by (clarsimp simp: mem_read_hp'_def split: split_if_asm)
+
+
+
+lemma [simp]:
+  "aval e s = Some v \<Longrightarrow>  aval e (s\<lparr>incon_set := {av \<in> incon_set s. fst av \<noteq> asid s}\<rparr>) = Some v"
+ by (induct e arbitrary: v; clarsimp split: option.splits; fastforce)
+
+(* apply (induct e arbitrary: v s)
+  apply (clarsimp)
+apply ( clarsimp split: option.splits)
+apply ( clarsimp split: option.splits)
+  
+  apply ( clarsimp split: option.splits) *)
+
+ 
 lemma flush_ASID_mem_write:
   "\<Turnstile> \<lbrace> \<lambda>s. aval lval s = Some vp \<and> aval rval s = Some v \<and> asid s = a \<and>  (a, vp) \<in> incon_set s \<and> mode s = Kernel \<and> 
       ptable_lift_m (heap s) (root s) (mode s) (Addr vp) = Some pp \<rbrace>  Flush (flushASID a) ;; lval ::= rval \<lbrace>\<lambda>s. heap s pp = Some v \<rbrace>"
-    by vcg
+  by vcgm
 
+lemma [simp]:
+  "mem_read_hp' (asid sa) (incon_set sa) (heap sa) (root sa) (Addr x2) = Some v
+                \<Longrightarrow> mem_read_hp' (asid sa) {av \<in> incon_set sa. fst av \<noteq> asid s \<and> snd av \<noteq> vp} (heap sa) (root sa) (Addr x2) = Some v"
+ by (clarsimp simp: mem_read_hp'_def split: split_if_asm)
+
+lemma  [simp]:
+  "aval e sa = Some v \<Longrightarrow>  aval e (sa\<lparr>incon_set := {av \<in> incon_set sa. fst av \<noteq> asid s \<and> snd av \<noteq> vp}\<rparr>) = Some v"
+ by (induct e arbitrary: v; clarsimp split: option.splits; fastforce)
 
 lemma flush_ASID_va_mem_write:
   "\<Turnstile> \<lbrace> \<lambda>s. aval lval s = Some vp \<and> aval rval s = Some v \<and>  asid s = a \<and> (asid s, vp) \<in> incon_set s \<and> mode s = Kernel \<and> 
       ptable_lift_m (heap s) (root s) (mode s) (Addr vp) = Some pp \<rbrace>  Flush (flushASIDva (asid s)  (Addr vp)) ;; lval ::= rval \<lbrace>\<lambda>s. heap s pp = Some v \<rbrace>"
-   by vcg
-
+  by vcgm
+ 
 
 
 end
