ROOT
@@ -13,18 +13,45 @@ session Word_Lib (AFP) in "Word_Lib" = "HOL-Word" +
 (* Collection of base theories that change rarely *)
 session L3_LIB = Word_Lib +
   theories
-  	"L3_Lib"
-	"PageTable_seL4_m"
+    "L3_Lib"
+    "PageTable_seL4_m"
 
 (* Main TLB and ARM model *)
 session ARM_TLB = L3_LIB +
   theories
     "MMU_ARM"
-	"Invalid_Ops"
-	"Program_Logic"
+    "Invalid_Ops"
+    "Update_ASID_Refine"
+    "Update_TTBR0_Refine"
+
+     
+
+(* Partial Model *)
+session ARM_Part = ARM_TLB +
+  theories
+    "PED_Cache"
+    "MMU_ARM_partial"
+        
+
+(* No_Fault Model *)
+session ARM_No_Fault = ARM_TLB +
+  theories
+    "MMU_ARM_Refine_No_Fault"
+   
+
+
 
 (* Case studies/examples on top of the model *)
 session ARM_TLB_Examples = ARM_TLB +
   theories
-    "Ins_Cycle"
-    "Ins_Cycle1"
+    "./ins_cycle/Ins_Cycle"
+    "/ins_cycle/IIns_Cycle1"
+
+
+
+session logic =  L3_LIB +
+   theories
+   "./logic/Boot"
+   "./logic/Kernel_Execution"
+   "./logic/Mode_Switch" 
+
